inital commit

AddPoly.ec
@@ -6,43 +6,52 @@ require import Group List AddList Ring AllCore IntDiv Bigalg DList DProd Distr A
   prime order cyclic group *)
 theory AddPoly.
 
-clone Bilinear.Bl as Bl.
-  
-import Bl.
+clone import Bilinear.Bl as Bl.
 
 clone IDomain as R with
-  type t <= GP.exp,
-  op zeror <= GP.ZModE.zero,
-  op oner <= GP.ZModE.one,
-  op   ( + ) <= GP.ZModE.( + ),
-  op   [ - ] <= GP.ZModE.([-]),
-  op   ( * ) <= GP.ZModE.( * ),
-  op   invr  <= GP.ZModE.inv,
-  pred   unit <= fun x => (x <>  GP.ZModE.zero),
-  lemma addrA <=  GP.ZModE.ZModpField.addrA,
-  lemma addrC  <= GP.ZModE.ZModpField.addrC,
-  lemma add0r <=  GP.ZModE.ZModpField.add0r,
-  lemma addNr <=  GP.ZModE.ZModpField.addNr,
-  lemma mulrA <=  GP.ZModE.ZModpField.mulrA,
-  lemma mulrC <=  GP.ZModE.ZModpField.mulrC,
-  lemma mul1r <=  GP.ZModE.ZModpField.mul1r,
-  lemma mulrDl <= GP.ZModE.ZModpField.mulrDl,
-  lemma oner_neq0 <= GP.ZModE.ZModpField.oner_neq0,
-  lemma mulVr <= GP.ZModE.ZModpField.mulVr,
-  lemma unitP <= GP.ZModE.ZModpField.unitP,
-  lemma unitout <= GP.ZModE.ZModpField.unitout,
-  lemma mulf_eq0 <= GP.ZModE.ZModpField.mulf_eq0.
+  type t <= ZP.exp,
+  op zeror <= ZP.ZModE.zero,
+  op oner <= ZP.ZModE.one,
+  op   ( + ) <= ZP.ZModE.( + ),
+  op   [ - ] <= ZP.ZModE.([-]),
+  op   ( * ) <= ZP.ZModE.( * ),
+  op   invr  <= ZP.ZModE.inv,
+  pred   unit <= fun x => (x <>  ZP.ZModE.zero),
+  lemma addrA <=  ZP.ZModE.ZModpField.addrA,
+  lemma addrC  <= ZP.ZModE.ZModpField.addrC,
+  lemma add0r <=  ZP.ZModE.ZModpField.add0r,
+  lemma addNr <=  ZP.ZModE.ZModpField.addNr,
+  lemma mulrA <=  ZP.ZModE.ZModpField.mulrA,
+  lemma mulrC <=  ZP.ZModE.ZModpField.mulrC,
+  lemma mul1r <=  ZP.ZModE.ZModpField.mul1r,
+  lemma mulrDl <= ZP.ZModE.ZModpField.mulrDl,
+  lemma oner_neq0 <= ZP.ZModE.ZModpField.oner_neq0,
+  lemma mulVr <= ZP.ZModE.ZModpField.mulVr,
+  lemma unitP <= ZP.ZModE.ZModpField.unitP,
+  lemma unitout <= ZP.ZModE.ZModpField.unitout,
+  lemma mulf_eq0 <= ZP.ZModE.ZModpField.mulf_eq0.
      
 clone Poly.Poly as BasePoly with
-  type coeff <- GP.exp,
- theory IDCoeff <- R.
+  type coeff <= ZP.exp,
+ theory IDCoeff <= R.
 
  import BasePoly.
- import R.
+ import ZP.ZModE.
 
- 
-  op prepolyCn (k   : int, c : GP.exp) = fun i => if 0 <= k /\ i = k then c else zeror.
-  lemma ispolyCn (k : int, c : GP.exp) : BasePoly.ispoly (prepolyCn k c).
+ (* poly to list *)
+  op listP (p : poly) = (map (fun i => p.[i]) (range 0 (deg p))).
+
+  lemma polyL_listP p : p = polyL (listP p).
+  proof.
+    apply poly_eqP. move => c hc. rewrite polyLE. case (c < size (range 0 (deg p))) => h.
+    rewrite (nth_map 0). trivial. simplify. rewrite nth_range. smt(@List). smt().
+    (* c is out of range *)
+    rewrite nth_default. smt(@List). apply gedeg_coeff. smt(@List).
+  qed.
+
+  (* create a polynomial which has constant c in term of order k *)
+  op prepolyCn (k   : int, c : ZP.exp) = fun i => if 0 <= k /\ i = k then c else zero.
+  lemma ispolyCn (k : int, c : ZP.exp) : BasePoly.ispoly (prepolyCn k c).
       proof.
       split=> @/prepolyCn [l lt0_l|].
         + case: (0 <= k); move => h; smt(@Int).
@@ -52,52 +61,46 @@ clone Poly.Poly as BasePoly with
     op polyCn k c = BasePoly.to_polyd (prepolyCn k c).
 
       
-  lemma polyCnE k c i : (polyCn k c).[i] = if 0 <= k /\ i = k then c else zeror.
+  lemma polyCnE k c i : (polyCn k c).[i] = if 0 <= k /\ i = k then c else zero.
       by rewrite coeffE 1:ispolyCn. qed.
     
-  lemma deg_polyCn c i: c <> zeror => 0 <= i => deg (polyCn i c) = i + 1.
+  lemma deg_polyCn c i: c <> zero => 0 <= i => deg (polyCn i c) = i + 1.
   proof.
       move => h h'. apply/degP=> //=; trivial. smt(). rewrite polyCnE. smt().
       move => i' hi. rewrite polyCnE. smt().
   qed.
 
   lemma lc_polyCn c i : 0 <= i => lc (polyCn i c) = c.
-  proof.
-    move => h. rewrite polyCnE. rewrite h. simplify. case (c = zeror) => h'. subst. smt(). rewrite deg_polyCn; trivial.
+      proof.
+    move => h. rewrite polyCnE. rewrite h. simplify. case (c = zero) => h'. subst. smt(). rewrite deg_polyCn; trivial.
   qed.
 
      lemma foldr_mkseq_bigi_eq f : forall j, 0 <= j => BigCf.BCA.bigi predT f 0 j =
-       foldr R.(+) zeror (mkseq f j).
-   proof.
-     apply intind. simplify. move => @/bigi @/range. simplify. rewrite iota0. smt(). rewrite BigCf.BCA.big_nil. simplify.
-     smt(@List).
-     (* inductive case *)
-     move => i ip ind_hyp. simplify. rewrite mkseqS. smt(). rewrite foldr_rcons. simplify.
-     have : f i + zeror = zeror + f i. smt(@GP.ZModE).  move => g. rewrite g. rewrite foldr_const. smt(@GP.ZModE).
-     smt(@GP.ZModE). rewrite -ind_hyp. move => @/bigi @/range. simplify. rewrite iotaSr. smt(). rewrite BigCf.BCA.big_rcons.
-     simplify. have : predT i = true. smt(). move => g'. rewrite g'. simplify. smt(@GP.ZModE).
+       foldr (+) zero (mkseq f j).
+    proof.
+      smt(@List @BigCf).
    qed.
     
-  lemma polyMCnE_0 p c : (p * polyCn 1 c).[0] = zeror.
+  lemma polyMCnE_0 p c : (p * polyCn 1 c).[0] = zero.
   proof.
     rewrite polyME. rewrite  foldr_mkseq_bigi_eq. smt(). simplify. rewrite mkseq1. simplify. rewrite polyCnE.
-    smt(@GP.ZModE).
+    smt(@ZP.ZModE).
   qed.
 
-  lemma  polyMCn_deg p c : c <> zeror => p <> poly0 => deg (p * polyCn 1 c) = deg p + 1.
+  lemma  polyMCn_deg p c : c <> zero => p <> poly0 => deg (p * polyCn 1 c) = deg p + 1.
   proof.
-    move => h h'. rewrite degM_proper. apply mulf_neq0. smt(lc_eq0). rewrite lc_polyCn. smt(). trivial.
+    move => h h'. rewrite degM_proper. apply ZModpField.mulf_neq0. smt(lc_eq0). rewrite lc_polyCn. smt(). trivial.
     rewrite deg_polyCn; trivial.
   qed.
 
-  lemma polyCn_poly0 i : polyCn i zeror = poly0.
+  lemma polyCn_poly0 i : polyCn i zero = poly0.
   proof.
     apply poly_eqP => c hc. rewrite polyCnE. case(0 <= i /\ c =i) => h. smt(poly0E). smt(poly0E). 
 qed.
 
   (* Intro a construction which builds a poynomial of order 2 or less, which is used for lagrange inter.  *)
-  op prepolyD2 (c1 c0 : GP.exp) = fun i => if i = 0 then c0 else (if i = 1 then c1 else zeror).
-  lemma ispolyD2 (c1 c0 : GP.exp) : BasePoly.ispoly (prepolyD2 c0 c1).
+  op prepolyD2 (c1 c0 : exp) = fun i => if i = 0 then c0 else (if i = 1 then c1 else zero).
+  lemma ispolyD2 (c1 c0 : exp) : BasePoly.ispoly (prepolyD2 c0 c1).
       proof.
       split=> @/prepolyD2 [l lt0_l|].
         + smt(@Int).
@@ -106,14 +109,14 @@ qed.
     
   op polyD2 c1 c0 = BasePoly.to_polyd (prepolyD2 c1 c0).
     
-   lemma polyD2E c1 c0 i : (polyD2 c1 c0).[i] =  if i = 0 then c0 else (if i = 1 then c1 else zeror).
+   lemma polyD2E c1 c0 i : (polyD2 c1 c0).[i] =  if i = 0 then c0 else (if i = 1 then c1 else zero).
        by rewrite coeffE 1:ispolyD2. qed.
      
-  lemma deg_polyD2 c1 c0 : c1 <> zeror => deg (polyD2 c1 c0) = 2.
+  lemma deg_polyD2 c1 c0 : c1 <> zero => deg (polyD2 c1 c0) = 2.
   proof.
     move => h. apply/degP=> //=; trivial. rewrite polyD2E. smt().
       move => i' hi. rewrite polyD2E. smt().
-qed.
+ qed.
 
   lemma deg_leq_polyD2 c1 c0 : deg (polyD2 c1 c0) <= 2.
   proof.
@@ -121,14 +124,14 @@ qed.
     rewrite g g'. simplify. trivial.
   qed.
 
-  lemma lc_polyD2 c1 c0 : c1 <> zeror => lc (polyD2 c1 c0) = c1.
+  lemma lc_polyD2 c1 c0 : c1 <> zero => lc (polyD2 c1 c0) = c1.
   proof.
     move => h. rewrite polyD2E. rewrite deg_polyD2; trivial.
   qed.
  
-  lemma  polyMD2_deg p c1 c0 : c1 <> zeror => p <> poly0 => deg (p * polyD2 c1 c0) = deg p + 1.
+  lemma  polyMD2_deg p c1 c0 : c1 <> zero => p <> poly0 => deg (p * polyD2 c1 c0) = deg p + 1.
   proof.
-    move => h h'. rewrite degM_proper. apply mulf_neq0. smt(lc_eq0). rewrite lc_polyD2; trivial. 
+    move => h h'. rewrite degM_proper. apply ZModpField.mulf_neq0. smt(lc_eq0). rewrite lc_polyD2; trivial. 
     rewrite deg_polyD2; trivial.
   qed.
 
@@ -138,7 +141,7 @@ qed.
     simplify. smt(@R).
   qed.
 
-  lemma polyD2_polyC c0 : polyD2 zeror c0 = polyC c0. 
+  lemma polyD2_polyC c0 : polyD2 zero c0 = polyC c0. 
   proof.
     apply poly_eqP => c hc. rewrite polyCE polyD2E. smt().
   qed.
@@ -146,73 +149,73 @@ qed.
   (* Inital poly lemmas *)
 
  lemma peval_simp (m :poly) a :
-    peval m a = foldr ( + )%R zeror
+    peval m a = foldr ( +) zero
       (mkseq (fun i => ( * )  m.[i] (exp a i))
         (deg m + 1)).
-   proof.
-     move => @/peval @/big. apply eq_foldr; trivial. apply (eq_from_nth zeror).
-     smt(@List). move => i h. rewrite filter_predT. rewrite filter_predT in h.
-     rewrite size_map in h. rewrite size_range in h. rewrite nth_mkseq. smt().
-     rewrite nth_mkseq. smt(). smt().
+  proof.
+     rewrite -foldr_mkseq_bigi_eq. smt(ge0_deg). move => @/peval. trivial.
  qed.
 
-  lemma peval_simp_gen (m :poly) a j : deg m <= j =>
-    peval m a = foldr ( + )%R zeror
+  lemma peval_simp_gen (m :poly) a j : deg m + 1 <= j  =>
+    peval m a = foldr ( + ) zero
       (mkseq (fun i => ( * )  m.[i] (exp a i)) j).
-   proof.
-     move => h. move => @/peval @/big. apply eq_foldr_trunc; trivial. smt(@R). smt(@R). smt(@R).
-     move => i hi.
-     (* case where the exp is non-zero *)
-     case (i < deg m) => g. rewrite (nth_mkseq). smt(@List). rewrite (nth_map 0). smt(@List). simplify. smt(@List).
-     case (i = deg m) => g'. rewrite (nth_map 0). smt(@List).  case(j = deg m) => g''. rewrite eq_sym. rewrite nth_default.
-     smt(@List). rewrite gedeg_coeff. smt(@List). smt(@R). rewrite nth_mkseq. smt(). simplify. smt(@List). rewrite nth_mkseq.
-     smt(@List). rewrite (nth_default). smt(@List). simplify. rewrite gedeg_coeff. smt(). smt(@R).
+  proof.
+    rewrite peval_simp. move => h. apply foldr_eq_partL; trivial. smt(@R). smt(@R). smt(@R). smt(@List).
+    (* first part equal *) smt(@List).
+    (* zero_tail *) apply (all_nth _ zero). move => i hi. simplify. rewrite nth_drop. smt(@List). smt().  
+    rewrite nth_mkseq. smt(@List). simplify. rewrite gedeg_coeff. smt(@List). smt(@R).
   qed.
  
   lemma polyL0 :polyL [] = poly0.
     proof.
       apply poly_eqP. move => c h. rewrite polyCE. rewrite polyLE. smt(@BasePoly). 
-    qed.
-
+  qed.
+    
   (* If you evaluate the zero polnomial at any point you get zero *)
-  lemma peval0 a : peval poly0 a = zeror.
+  lemma peval0 a : peval poly0 a = zero.
   proof.    
     move => @/peval. rewrite BigCf.BCA.big1. move => i h.
     simplify. rewrite poly0E. smt(@R). smt(@R).
   qed.
 
-  lemma exp_dumb : forall i, 0 <= i => exp zeror (1 + i) = zeror.
+  lemma exp_dumb : forall i, 0 <= i => exp zero (1 + i) = zero.
   proof.
-    apply intind. smt(expr1). move => i g0 h. simplify. have : i +2 = i + 1 + 1. smt(). move => g. rewrite g.
-    rewrite exprS. smt(). smt(@GP.ZModE).
+    apply intind. smt(R.expr1). move => i g0 h. simplify. have : i +2 = i + 1 + 1. smt(). move => g. rewrite g.
+    smt(@ZP.ZModE).
 qed.
 
-  
+lemma lc_deg p : lc p <> zero => deg p <> 0.
+    smt(@BasePoly).
+  qed.
+    
   lemma degD_proper p q :
-      lc p + lc q <> zeror => deg (p+q) = max (deg p)(deg q).
+      lc p + lc q <> zero => deg (p+q) = max (deg p)(deg q).
   proof.
-    move => h. apply degP; smt(@BasePoly).
+  move => h. apply degP. have : lc p <> zero \/ lc q <> zero. smt(@BasePoly).
+    move => h'. smt(lc_deg BasePoly.ge0_deg). admit. smt(@BasePoly).
   qed.
 
-  lemma degD_inproper (p q : poly) : deg (p+ q) <> max (deg p) (deg q) => deg p = deg q /\ lc p + lc q = zeror.
+  lemma degD_inproper (p q : poly) : deg (p+ q) <> max (deg p) (deg q) =>
+    deg p = deg q /\ lc p + lc q = zero.
    proof.
-     move => h. have : deg p = deg q. smt(@BasePoly). move => h'. split. trivial. smt(@BasePoly).
+     move => h. have : deg p = deg q. admit. move => h'. split. trivial. admit.
  qed.
 
-  lemma peval_id p : peval p zeror = p.[0].
+  lemma peval_id p : peval p zero = p.[0].
    proof.    
      rewrite peval_simp. rewrite mkseqSr. smt(@BasePoly). simplify.  rewrite foldr_id.
-     smt(@GP.ZModE). rewrite (all_nth _ GP.ZModE.zero).
+     smt(@ZP.ZModE). rewrite (all_nth _ ZP.ZModE.zero).
      move => i h. simplify. rewrite nth_mkseq. smt(@List). move => @/(\o). rewrite exp_dumb. smt(@List).
-     smt(@GP.ZModE). rewrite expr0. smt(@GP.ZModE).
+     smt(@ZP.ZModE). rewrite ZModpField.expr0. smt(@ZP.ZModE).
   qed.
 
   lemma peval_polyC a b : peval (polyC a) b = a.
   proof.
-    rewrite peval_simp. case (a = zeror); move => h. have : deg (polyC a) = 0. smt(@BasePoly).
-    move => h'. rewrite h'. rewrite mkseq1. simplify. smt(@BasePoly @GP.ZModE).
+    rewrite peval_simp. case (a = zero); move => h. have : deg (polyC a) = 0. smt(@BasePoly).
+    move => h'. rewrite h'. rewrite mkseq1. simplify. smt(@BasePoly @ZP.ZModE).
     have : deg (polyC a) = 1. smt(@BasePoly). move => h'. rewrite h'. rewrite mkseqS. smt().
-    rewrite mkseq1. simplify. rewrite polyCE. rewrite polyCE. simplify. rewrite expr0. smt(@BasePoly @GP.ZModE).
+    rewrite mkseq1. simplify. rewrite polyCE. rewrite polyCE. simplify. rewrite ZModpField.expr0.
+    smt(@BasePoly @ZP.ZModE).
   qed.
 
   lemma polyC_peval p i : deg p < 2 => polyC (peval p i) = p.
@@ -227,73 +230,50 @@ qed.
   proof.
     rewrite peval_simp. have : deg (X) = 2. smt(@BasePoly). move => h. rewrite h.
     rewrite mkseqS. smt(). have : 2 = 1 + 1. smt(). move => h''. rewrite h''. rewrite mkseqS. smt(). rewrite mkseq1.
-    simplify. rewrite polyXE. rewrite polyXE. rewrite polyXE. simplify. rewrite expr1. smt(@GP.ZModE).
-  qed.
-
-  
-  lemma peval_add_sub i j :  forall p p' a, i = deg p => j = deg p' => peval p a + peval p' a = peval (p + p') a.
-  proof.
-    wlog: i j / i <= j => [wlog p p' a h h'|le_ij]. case (i <= j); move => g. apply (wlog i j); trivial.
-    have : p + p' = p' + p. smt(@BasePoly). move => g'. rewrite g'. rewrite -(wlog j i); trivial. smt().  smt(@GP.ZModE).
-    (* we have discharged the general principial and now need to show the base case holds *)
-     move => p p' a h h'. rewrite peval_simp. rewrite peval_simp. rewrite peval_simp. rewrite foldr_add_distr_sub.
-    smt(@GP.ZModE). smt(@GP.ZModE).   smt(@GP.ZModE). smt(@List).
-    rewrite size_mkseq. rewrite size_mkseq. apply eq_foldr_trunc.   smt(@GP.ZModE).   smt(@GP.ZModE).   smt(@GP.ZModE).
-    move => i0 h''. rewrite size_mkseq in h''.
-    rewrite size_mkseq in h''. simplify. case (deg (p+p') = max (deg p)(deg p')); move => h'''.
-    (* main case *)
-    rewrite nth_mkseq. smt(@Int @BasePoly). rewrite nth_mkseq. smt(@Int). simplify.
-    rewrite polyDE. case (i0 < deg p + 1); move => g. rewrite nth_mkseq. smt(). rewrite nth_mkseq. smt(). simplify.
-    smt(@GP.ZModE). rewrite nth_default. smt(@List). rewrite nth_mkseq. smt(@Int @BasePoly). simplify.
-    rewrite (gedeg_coeff p). smt(). smt(@GP.ZModE).
-    (* annyoing case *)
-    have : deg (p + p') <> max (deg p) (deg p'). trivial. move => g. apply degD_inproper in h'''. rewrite nth_mkseq.
-    smt(@BasePoly). simplify. rewrite nth_mkseq. smt(@BasePoly). rewrite nth_mkseq. smt(@BasePoly). simplify.
-    case (i0 < deg(p + p') + 1); move => g'. rewrite nth_mkseq. smt(). smt(@BasePoly @GP.ZModE).
-    rewrite nth_default. smt(@List). have : (p + p').[i0] = zeror. smt(@BasePoly @GP.ZModE). move => g''.
-    have : p.[i0] * exp a i0 + p'.[i0] * exp a i0 = (p.[i0] + p'.[i0]) * exp a i0. smt(@GP.ZModE). move => g'''. rewrite g'''.
-    smt(@BasePoly @GP.ZModE).
+    simplify. rewrite polyXE. rewrite polyXE. rewrite polyXE. simplify. rewrite ZModpField.expr1. smt(@ZP.ZModE).
 qed.
 
-  lemma peval_add p p' a : peval p a + peval p' a = peval (p + p') a.
-    apply (peval_add_sub (deg p)(deg p')); trivial.
-    qed.
-    
+lemma peval_add p p' a : peval p a + peval p' a = peval (p + p') a.
+    rewrite !(peval_simp_gen _ _ (max (deg p + 1)(deg p' + 1))). smt(). smt(). smt(degD).
+    rewrite -foldr_add_distr_f. smt(@R). smt(@R). smt(@R). smt(ge0_deg). congr.
+    congr. simplify. rewrite fun_ext. move => i. rewrite polyDE. admit.
+  qed.
+  
   lemma peval_mul p a b : peval p a * b = peval (b ** p) a.
   proof.
-    rewrite !peval_simp. rewrite dis_mul_add. smt(@GP.ZModE). smt(@GP.ZModE). apply foldr_eq_partR. smt(@GP.ZModE).
-    smt(@GP.ZModE). smt(@GP.ZModE). smt(@GP.ZModE). smt(@List @BasePoly). apply (eq_from_nth zeror).
-    smt(@List @BasePoly). move => i hi. rewrite size_mkseq in hi. rewrite nth_mkseq. smt(@BasePoly).
-    rewrite nth_take. smt(@List @BasePoly).  smt(@List @BasePoly). rewrite (nth_map zeror).  smt(@List @BasePoly).
-    rewrite nth_mkseq.  smt(@List @BasePoly).  simplify. rewrite polyZE. smt(@GP.ZModE).
-    apply (all_nth _ zeror). move => i hi.  rewrite size_drop in hi. smt(@List @BasePoly). rewrite size_map in hi.
-    rewrite !size_mkseq in hi. rewrite nth_drop. smt(@List @BasePoly). smt(). simplify. rewrite (nth_map zeror).
-    smt(@List @BasePoly). rewrite nth_mkseq. smt(@List @BasePoly). rewrite size_mkseq. simplify.
-    case (b = zeror) => g. smt(@GP.ZModE). rewrite gedeg_coeff. rewrite scalepE.
-    have : deg (polyC b * p) = deg p. rewrite degM_proper. smt(@BasePoly @GP.ZModE). smt(@BasePoly).
-    move => h.  rewrite h. smt(). smt(@GP.ZModE).
-  qed.
+    rewrite !peval_simp. rewrite dis_mul_add. smt(@ZP.ZModE). smt(@ZP.ZModE).
+    case (R.lreg b) => h. rewrite degZ_lreg; trivial. congr. rewrite R.lregP in h. rewrite map_mkseq. congr.
+    rewrite fun_ext => i. simplify. rewrite polyZE. smt(@ZP.ZModE).
+    rewrite R.lregP in h. rewrite !foldr_id; trivial. smt(@ZP.ZModE). apply (all_nth _ zero) => i hi.
+    simplify. rewrite (nth_map zero). smt(@List). simplify. smt(@ZP.ZModE).
+    smt(@ZP.ZModE). apply (all_nth _ zero) => i hi. simplify. rewrite nth_mkseq. smt(@Poly @List). simplify.
+    rewrite polyZE. smt(@ZP.ZModE).
+ qed.
 
   lemma poly_sum_nth x i : (foldr BasePoly.(+) poly0 x).[i] =
-   foldr R.(+) zeror (map (fun p=> p.[i]) x).
+   foldr R.(+) zero (map (fun p=> p.[i]) x).
   proof.
     elim x. simplify. smt(@BasePoly). move => x l ind_hyp. simplify. rewrite -ind_hyp. smt(@BasePoly).
   qed.
   
-  lemma peval_sum phis x : peval (foldr BasePoly.(+) poly0 phis) x = foldr R.(+) zeror (map (fun phi => peval phi x) phis).
+  lemma peval_sum phis x : peval (foldr BasePoly.(+) poly0 phis) x = foldr(+) zero (map (fun phi => peval phi x) phis).
   proof.
     elim phis. simplify. apply peval0. move => x0 l ind_hyp. simplify. rewrite -peval_add. smt().
   qed.
+
+  (** Polished up this point *)
   
   lemma peval_neg_sub p a : - peval (polyL p) a = peval (-(polyL p)) a.
-  proof.
+      proof.
+        admit.
+        (*
     rewrite peval_simp. rewrite peval_simp.
     have : mkseq (fun (i : int) => (- polyL p).[i] * exp a i) (deg (- polyL p) + 1) =
-    map (fun (a : GP.exp) => - a) (mkseq (fun i => (polyL p).[i] * exp a i) (deg (polyL p) + 1)).
-    apply (eq_from_nth zeror). smt(@List @BasePoly). move => i h. rewrite (nth_map zeror).
+    map (fun (a : exp) => - a) (mkseq (fun i => (polyL p).[i] * exp a i) (deg (polyL p) + 1)).
+    apply (eq_from_nth zero). admit. admit. move => i h. rewrite (nth_map zero).
     smt(@List @BasePoly). rewrite nth_mkseq. smt(@BasePoly @List). rewrite nth_mkseq.
     smt(@List @BasePoly). simplify. rewrite polyLE. rewrite polyNE. rewrite polyLE.
-    smt(@GP.ZModE). move => h. rewrite h. apply dis_neg; smt(@GP.ZModE).
+    smt(@ZP.ZModE). move => h. rewrite h. apply dis_neg; smt(@ZP.ZModE).*)
   qed.
 
   lemma peval_neg p a : - peval p a = peval (-p) a.
@@ -302,7 +282,7 @@ qed.
   qed.
 
   lemma Xi_eval i a : peval (X - polyC i) a = a - i. rewrite -polyCN. rewrite -peval_add.
-    rewrite peval_X. rewrite peval_polyC. smt(@GP.ZModE).
+    rewrite peval_X. rewrite peval_polyC. smt(@ZP.ZModE).
     qed.
 
   
@@ -310,32 +290,33 @@ qed.
    proof.
       case (p = poly0); move => h.
      (* stupid case *)
-     rewrite h. smt(peval0 @BasePoly @GP.ZModE).
+     rewrite h. smt(peval0 @BasePoly @ZP.ZModE).
      (* resume *)
      rewrite peval_simp. rewrite peval_simp. rewrite mkseqSr. smt(@BasePoly). simplify.
-     have : forall b, (p * X).[0] * exp a 0 + b = b. rewrite expr0. have :  (p * X).[0] = zeror. smt(@BasePoly @GP.ZModE).
-     move => h'. rewrite h'. smt(@GP.ZModE). move => h'. rewrite h'. rewrite dis_mul_add. smt(@GP.ZModE). smt(@GP.ZModE).
-     apply eq_foldr; trivial. apply (eq_from_nth zeror). smt(@List @BasePoly). move => i ip. rewrite nth_mkseq. smt(@List).
-     rewrite (nth_map zeror). smt(@List @BasePoly). rewrite nth_mkseq. smt(@List @BasePoly). move => @/(\o). simplify.
-     rewrite polyMXE. have : 1 + i = i + 1. smt(). move => g. rewrite g. rewrite exprS. smt(). smt(@GP.ZModE).
+     have : forall b, (p * X).[0] * exp a 0 + b = b. rewrite ZModpField.expr0.
+     have :  (p * X).[0] = zero. smt(@BasePoly @ZP.ZModE).
+     move => h'. rewrite h'. smt(@ZP.ZModE). move => h'. rewrite h'. rewrite dis_mul_add. smt(@ZP.ZModE). smt(@ZP.ZModE).
+     apply eq_foldr; trivial. apply (eq_from_nth zero). smt(@List @BasePoly). move => i ip. rewrite nth_mkseq. smt(@List).
+     rewrite (nth_map zero). smt(@List @BasePoly). rewrite nth_mkseq. smt(@List @BasePoly). move => @/(\o). simplify.
+     rewrite polyMXE. have : 1 + i = i + 1. smt(). move => g. rewrite g. rewrite ZModpField.exprS. smt(). smt(@ZP.ZModE).
  qed.
 
  lemma polyM_polyCn p c i : 0 <= i => (p * polyCn 1 c).[i + 1] = p.[i] * c.
  proof.
-   move => h. rewrite polyME. rewrite foldr_mkseq_bigi_eq. smt(). rewrite (foldr_id_nth_mkseq _ _ _ i). smt(@GP.ZModE).
-   smt(@GP.ZModE). smt(@GP.ZModE). smt().
-   apply (all_nth _ zeror) => i0 hi0. rewrite nth_mkseq. smt(@List). simplify. rewrite polyCnE. smt(@R @List).
-   apply (all_nth _ zeror) => i0 hi0. rewrite nth_mkseq. smt(@List). simplify. rewrite polyCnE. smt(@R @List).
+   move => h. rewrite polyME. rewrite foldr_mkseq_bigi_eq. smt(). rewrite (foldr_id_nth_mkseq _ _ _ i). smt(@ZP.ZModE).
+   smt(@ZP.ZModE). smt(@ZP.ZModE). smt().
+   apply (all_nth _ zero) => i0 hi0. rewrite nth_mkseq. smt(@List). simplify. rewrite polyCnE. smt(@R @List).
+   apply (all_nth _ zero) => i0 hi0. rewrite nth_mkseq. smt(@List). simplify. rewrite polyCnE. smt(@R @List).
    simplify. smt(polyCnE).
  qed.
 
-lemma polyM_polyD2 p c1 c0 i : 0 <= i => c1 <> zeror => (p * polyD2 c1 c0).[i + 1] =
+lemma polyM_polyD2 p c1 c0 i : 0 <= i => c1 <> zero => (p * polyD2 c1 c0).[i + 1] =
     (p.[i] * c1) + (p.[i + 1] * (polyD2 c1 c0).[0]).
  proof.
    move => h h'. rewrite polyME. rewrite foldr_mkseq_bigi_eq. smt(). rewrite mkseqS. smt(). rewrite mkseqS. smt(). 
- move => @/(\o). simplify. rewrite !foldr_rcons. have : forall a b, foldr R.(+) a b = a + (foldr R.(+) zeror b). move => a b.
+ move => @/(\o). simplify. rewrite !List.foldr_rcons. have : forall a b, foldr R.(+) a b = a + (foldr R.(+) zero b). move => a b.
    elim b. smt(@R). move => x l ind_hyp. smt(@R).
-   move => g. rewrite g.  rewrite foldr_id. smt(@GP.ZModE). apply (all_nth _ zeror) => i0 hi0. rewrite nth_mkseq. smt(@List).
+   move => g. rewrite g.  rewrite foldr_id. smt(@ZP.ZModE). apply (all_nth _ zero) => i0 hi0. rewrite nth_mkseq. smt(@List).
    simplify. rewrite polyD2E. smt(@R @List). rewrite polyD2E. simplify. have : i + 1 - i <> 0. smt(). move => g'. rewrite !g'.
    have : i + 1 - i = 1. smt(). move => g''. rewrite g''. simplify. smt(@R).
  qed.
@@ -344,22 +325,23 @@ lemma polyM_polyD2 p c1 c0 i : 0 <= i => c1 <> zeror => (p * polyD2 c1 c0).[i + 
    proof.
      case (p = poly0); move => h.
      (* stupid case *)
-     rewrite h. smt(peval0 @BasePoly @GP.ZModE).
+     rewrite h. smt(peval0 @BasePoly @ZP.ZModE).
      (* second stupid case *)
-     case (c = zeror) => h'. subst. rewrite polyCn_poly0. rewrite IDPoly.mulrC. rewrite mul0p. rewrite peval0. smt(@R).
+     case (c = zero) => h'. subst. rewrite polyCn_poly0. rewrite IDPoly.mulrC. rewrite mul0p. rewrite peval0. smt(@R).
      (* resume *)
      rewrite peval_simp. rewrite peval_simp. rewrite polyMCn_deg; trivial. rewrite mkseqSr. smt(@BasePoly). simplify.
-     have : forall b, (p * polyCn 1 c).[0] * exp a 0 + b = b. rewrite expr0. rewrite polyMCnE_0.  smt(@GP.ZModE). move => g'.
-     rewrite g'. rewrite dis_mul_add. smt(@GP.ZModE). smt(@GP.ZModE). rewrite dis_mul_add. smt(@GP.ZModE). smt(@GP.ZModE).
-     apply eq_foldr; trivial. apply (eq_from_nth zeror). smt(@List @BasePoly). move => i ip. rewrite nth_mkseq. smt(@List).
-     rewrite (nth_map zeror). smt(@List @BasePoly). rewrite (nth_map zeror). smt(@List @BasePoly). rewrite nth_mkseq.
-     smt(@List @BasePoly). move => @/(\o). simplify. have : 1 + i = i + 1. smt(). move => g. rewrite g. rewrite exprS. smt().
+     have : forall b, (p * polyCn 1 c).[0] * exp a 0 + b = b. rewrite ZModpField.expr0. rewrite polyMCnE_0.  smt(@ZP.ZModE).
+   move => g'.
+     rewrite g'. rewrite dis_mul_add. smt(@ZP.ZModE). smt(@ZP.ZModE). rewrite dis_mul_add. smt(@ZP.ZModE). smt(@ZP.ZModE).
+     apply eq_foldr; trivial. apply (eq_from_nth zero). smt(@List @BasePoly). move => i ip. rewrite nth_mkseq. smt(@List).
+     rewrite (nth_map zero). smt(@List @BasePoly). rewrite (nth_map zero). smt(@List @BasePoly). rewrite nth_mkseq.
+     smt(@List @BasePoly). move => @/(\o). simplify. have : 1 + i = i + 1. smt(). move => g. rewrite g. rewrite ZModpField.exprS.
+     smt().
      rewrite polyM_polyCn. smt(). smt(@R).
  qed.
-
      
    lemma polyM_eq p q k : BigCf.BCA.bigi predT (fun i => p.[i] * q.[k-i]) 0 (k+1) =
-       foldr R.(+) zeror (mkseq (fun i => p.[i] * q.[k-i]) (k+1)).
+       foldr (+) zero (mkseq (fun i => p.[i] * q.[k-i]) (k+1)).
    proof.
      case (0 <= k + 1); move => h. apply foldr_mkseq_bigi_eq. smt(). move => @/bigi @/range. rewrite iota0. smt().
      rewrite BigCf.BCA.big_nil. rewrite mkseq0_le. smt(). smt().
@@ -368,69 +350,66 @@ lemma polyM_polyD2 p c1 c0 i : 0 <= i => c1 <> zeror => (p * polyD2 c1 c0).[i + 
       
    lemma polyM_polyC p i j: 0<= j =>  (p * polyC i).[j] = p.[j] * i.
    proof.
-     move => h. rewrite polyME. rewrite polyM_eq. simplify. rewrite mkseqS; trivial. simplify. rewrite foldr_rcons.
-     have : p.[j] * (polyC i).[0] + zeror = zeror + p.[j] * (polyC i).[0]. smt(@GP.ZModE). move => h'. rewrite h'.
-     rewrite foldr_const. smt(@GP.ZModE). smt(@GP.ZModE). rewrite foldr_id.  smt(@GP.ZModE). apply (all_nth _ zeror).
-     move => s ps. simplify. rewrite nth_mkseq. smt(@List). simplify. rewrite polyCE. simplify. have : j - s <> 0.
-     smt(@List). move => g. rewrite g. simplify. smt(@GP.ZModE). smt(@BasePoly @GP.ZModE). 
+     move => h. rewrite polyME. rewrite polyM_eq. simplify. rewrite mkseqS; trivial. simplify. rewrite List.foldr_rcons.
+     rewrite R.addrC. rewrite foldr_const.  smt(@ZP.ZModE). smt(@ZP.ZModE). rewrite foldr_id.  smt(@ZP.ZModE).
+     apply (all_nth _ zero). move => s ps. simplify. rewrite nth_mkseq. smt(@List). simplify. rewrite polyCE.
+     simplify. have : j - s <> 0. smt(@List). move => g. rewrite g. simplify. smt(@ZP.ZModE). smt(@BasePoly @ZP.ZModE). 
    qed.
-
  
     lemma peval_polyM_C p a i : peval (p * polyC i) a = peval p a * i.
    proof.
-     rewrite peval_simp. rewrite peval_simp.  case (i = zeror); move => h. 
+     rewrite peval_simp. rewrite peval_simp.  case (i = zero); move => h. 
      (* special case *)
-     rewrite h. have : deg (p * polyC zeror) + 1 = 1. smt(@BasePoly). move => h'. rewrite h'. rewrite mkseq1.
-     simplify. smt(@BasePoly @GP.ZModE).
+     rewrite h. have : deg (p * polyC zero) + 1 = 1. smt(@BasePoly). move => h'. rewrite h'. rewrite mkseq1.
+     simplify. smt(@BasePoly @ZP.ZModE).
      (* General case *)
-     rewrite dis_mul_add. smt(@GP.ZModE). smt(@GP.ZModE). apply eq_foldr; trivial.
-     apply (eq_from_nth zeror). rewrite size_mkseq. rewrite size_map. rewrite size_mkseq.  smt(@BasePoly).
-     move => j jp. rewrite nth_mkseq. smt(@List). rewrite (nth_map zeror). smt(@List @BasePoly). rewrite nth_mkseq.
-     smt(@List @BasePoly). simplify. rewrite polyM_polyC. smt(). smt(@GP.ZModE).
+     rewrite dis_mul_add. smt(@ZP.ZModE). smt(@ZP.ZModE). apply eq_foldr; trivial.
+     apply (eq_from_nth zero). rewrite size_mkseq. rewrite size_map. rewrite size_mkseq.  smt(@BasePoly).
+     move => j jp. rewrite nth_mkseq. smt(@List). rewrite (nth_map zero). smt(@List @BasePoly). rewrite nth_mkseq.
+     smt(@List @BasePoly). simplify. rewrite polyM_polyC. smt(). smt(@ZP.ZModE).
   qed.
  
   lemma peval_polyM_polyD2 p c1 c0 a: peval (p * (polyD2 c1 c0)) a = peval p a * c1 * a + peval p a * c0.
-   proof.
+  proof.
      case (p = poly0); move => h.
      (* stupid case *)
-     rewrite h. smt(peval0 @BasePoly @GP.ZModE).
+     rewrite h. smt(peval0 @BasePoly @ZP.ZModE).
      (* second stupid case *)
-     case (c1 = zeror) => h'. subst. rewrite polyD2_polyC. rewrite peval_polyM_C. smt(@R).
+     case (c1 = zero) => h'. subst. rewrite polyD2_polyC. rewrite peval_polyM_C. smt(@R).
       (* resume *)
      rewrite !peval_simp. rewrite polyMD2_deg; trivial. 
      (* seq equal *)
-     rewrite dis_mul_add.  smt(@GP.ZModE). smt(@GP.ZModE). rewrite dis_mul_add.  smt(@GP.ZModE). smt(@GP.ZModE).
-     rewrite (dis_mul_add _ _ _ _ c0).  smt(@GP.ZModE). smt(@GP.ZModE). rewrite mkseqSr. smt(@BasePoly).
-     rewrite (map_mkseq (fun (x : GP.exp) => x * c0)).
-     rewrite (mkseqSr ((fun (x : GP.exp) => x * c0) \o fun (i : int) => p.[i] * exp a i)). smt(@BasePoly). simplify.
-     have: forall (a b c d e : GP.exp), a = d => b = c + e => a + b = c + (d + e). smt(@GP.ZModE). move => g'. apply g'.
-     move => @/(\o). rewrite expr0. rewrite polyMD2_0. smt(@R). have : forall (a b : GP.exp), a + b = b + a. smt(@GP.ZModE).
-     move => g''. rewrite g''. rewrite foldr_add_distr_sub. smt(@GP.ZModE). smt(@GP.ZModE). smt(@GP.ZModE).
+     rewrite dis_mul_add.  smt(@ZP.ZModE). smt(@ZP.ZModE). rewrite dis_mul_add.  smt(@ZP.ZModE). smt(@ZP.ZModE).
+     rewrite (dis_mul_add _ _ _ _ c0).  smt(@ZP.ZModE). smt(@ZP.ZModE). rewrite mkseqSr. smt(@BasePoly).
+     rewrite (map_mkseq (fun (x : ZP.exp) => x * c0)).
+     rewrite (mkseqSr ((fun (x : ZP.exp) => x * c0) \o fun (i : int) => p.[i] * exp a i)). smt(@BasePoly). simplify.
+     have: forall (a b c d e : ZP.exp), a = d => b = c + e => a + b = c + (d + e). smt(@ZP.ZModE). move => g'. apply g'.
+     move => @/(\o). rewrite ZModpField.expr0. rewrite polyMD2_0. smt(@R). rewrite R.addrC.
+     rewrite foldr_add_distr_sub. smt(@ZP.ZModE). smt(@ZP.ZModE). smt(@ZP.ZModE).
      smt(@List). rewrite size_mkseq. rewrite size_map. rewrite size_map. rewrite size_mkseq. 
-     apply eq_foldr; trivial. apply (eq_from_nth zeror). smt(@List @BasePoly). move => i ip. rewrite nth_mkseq. smt(@List).
-     rewrite (nth_mkseq zeror). smt(@List @BasePoly). simplify.  rewrite (nth_map zeror). smt(@List @BasePoly). 
-     rewrite (nth_map zeror). smt(@List @BasePoly). move => @/(\o). simplify.  have : 1 + i = i + 1. smt(). move => g'''. 
+     apply eq_foldr; trivial. apply (eq_from_nth zero). smt(@List @BasePoly). move => i ip. rewrite nth_mkseq. smt(@List).
+     rewrite (nth_mkseq zero). smt(@List @BasePoly). simplify.  rewrite (nth_map zero). smt(@List @BasePoly). 
+     rewrite (nth_map zero). smt(@List @BasePoly). move => @/(\o). simplify.  have : 1 + i = i + 1. smt(). move => g'''. 
      (* end case *)
      case (i = deg p) => h''. rewrite nth_default. smt(@List). rewrite nth_mkseq.  smt(@List @BasePoly). simplify.
      rewrite g'''. rewrite polyM_polyD2; trivial. smt(). smt(@R @BasePoly).
      (* normal case*)
-     rewrite nth_mkseq.  smt(@List @BasePoly).  rewrite nth_mkseq.  smt(@List @BasePoly). simplify.
-     rewrite g'''. rewrite polyM_polyD2; trivial. smt(). rewrite polyD2E. simplify. rewrite exprS. smt().
-     have : forall (a b c : GP.exp), (a + b) * c = (a * c) + (b * c). smt(@R). move => k. rewrite k. rewrite g''. congr.
-     smt(@R). smt(@R).
+     rewrite !nth_mkseq.  smt(@List @BasePoly). smt(@List @BasePoly). simplify. 
+    rewrite g'''. rewrite polyM_polyD2; trivial. smt(). rewrite polyD2E. simplify. rewrite ZModpField.exprS. smt().
+     rewrite ZModpField.mulrDl. smt(@R).
  qed.
  
-  lemma peval_polyCn_prod a bs (f : GP.exp -> GP.exp) :
+  lemma peval_polyCn_prod a bs (f : ZP.exp -> ZP.exp) :
     peval (foldr BasePoly.( * ) poly1 (map (fun x => polyCn 1 (f x)) bs)) a = 
-    foldr R.( * ) oner (map (fun x => a *x) (map f  bs)).
+    foldr R.( * ) one (map (fun x => a *x) (map f  bs)).
   proof.
     elim bs. simplify. rewrite peval_polyC. trivial. simplify. move => x l ind_hyp. rewrite IDPoly.mulrC.
     rewrite peval_polyM_polyCn. rewrite ind_hyp. smt(@R).
   qed.
   
-  lemma peval_polyD2_prod a bs (f f' : GP.exp -> GP.exp) :
+  lemma peval_polyD2_prod a bs (f f' : ZP.exp -> ZP.exp) :
     peval (foldr BasePoly.( * ) poly1 (map (fun x => polyD2 (f x) (f' x)) bs)) a = 
-    foldr R.( * ) oner (map (fun (x : GP.exp*GP.exp)  => a * x.`1 + x.`2 ) (map (fun x => (f x, f' x))  bs)). 
+    foldr R.( * ) one (map (fun (x : ZP.exp*ZP.exp)  => a * x.`1 + x.`2 ) (map (fun x => (f x, f' x))  bs)). 
   proof.
     elim bs. simplify. rewrite peval_polyC. trivial. simplify. move => x l ind_hyp. rewrite IDPoly.mulrC.
     rewrite peval_polyM_polyD2. rewrite ind_hyp. smt(@R).
@@ -441,17 +420,16 @@ lemma polyM_polyD2 p c1 c0 i : 0 <= i => c1 <> zeror => (p * polyD2 c1 c0).[i + 
   proof.
     have: p * (X - polyC i) = p * X - p * (polyC i). smt(@BasePoly). move => h. rewrite h.
     rewrite -peval_add. rewrite -peval_add. rewrite -peval_neg. rewrite -peval_neg.
-    rewrite peval_X. rewrite peval_polyC. rewrite peval_polyM_C. rewrite peval_polyM_X. smt(@GP.ZModE).
+    rewrite peval_X. rewrite peval_polyC. rewrite peval_polyM_C. rewrite peval_polyM_X. smt(@ZP.ZModE).
   qed.
 
-  lemma peval_Xi_prod js f i : peval (foldr BasePoly.( * ) poly1 (map (fun (x : GP.exp) => X - polyC (f x)) js)) i =
-      foldr R.( * ) oner (map (fun (x : GP.exp) => i - (f x)) js).
+  lemma peval_Xi_prod js f i : peval (foldr BasePoly.( * ) poly1 (map (fun (x : ZP.exp) => X - polyC (f x)) js)) i =
+      foldr R.( * ) one (map (fun (x : ZP.exp) => i - (f x)) js).
   proof.
     elim js. simplify. smt(peval_polyC). move => x l ind_hyp. simplify.  rewrite -ind_hyp.
     rewrite mulpC. rewrite -peval_over_Xi. rewrite -peval_add. rewrite peval_X. rewrite -peval_neg. rewrite peval_polyC.
     smt().  
-  qed.
-
+qed.
   
   lemma polyL_cat0 x l : of_poly (polyL (x :: l)) 0  = x.
   proof.  
@@ -467,31 +445,46 @@ lemma polyM_polyD2 p c1 c0 i : 0 <= i => c1 <> zeror => (p * polyD2 c1 c0).[i + 
       move => h. rewrite BasePoly.IDPoly.mulrC. rewrite (BasePoly.IDPoly.mulrC b c). apply poly_shift. trivial.
    qed.
    
-  lemma scale_1 c phi : c=oner => c ** phi = phi.
-  proof. move => h. rewrite h. apply poly_eqP. move => c0 ch. smt(@BasePoly @GP.ZModE). qed.
+  lemma scale_1 c phi : c=one => c ** phi = phi.
+  proof. move => h. rewrite h. apply poly_eqP. move => c0 ch. smt(@BasePoly @ZP.ZModE). qed.
 
   lemma Xi_0 i : (X - polyC i).[0] = - i. smt(@BasePoly). qed.
-  lemma Xi_1 i : (X - polyC i).[1] = oner. smt(@BasePoly). qed.
-  lemma Xi_0_add i : (X + polyC i).[0] = i. rewrite polyDE. smt(@BasePoly @GP.ZModE).  qed.
-  lemma Xi_1_add i : (X + polyC i).[1] = oner. smt(@BasePoly). qed.
+  lemma Xi_1 i : (X - polyC i).[1] = one. smt(@BasePoly). qed.
+  lemma Xi_0_add i : (X + polyC i).[0] = i. rewrite polyDE. smt(@BasePoly @ZP.ZModE).  qed.
+  lemma Xi_1_add i : (X + polyC i).[1] = one. smt(@BasePoly). qed.
 
   lemma Xi_neq_0 i : (X - polyC i) <> poly0. smt(@BasePoly). qed.
 
+  lemma Xi_polyD2 a :  X - polyC a = polyD2 one (-a).
+  proof.
+    apply poly_eqP. move => c hc. rewrite !polyD2E. case(1 < c) => h. smt(@BasePoly @ZP.ZModE).
+    case (c = 0) => h'. smt(@BasePoly @ZP.ZModE). have : (c = 1). smt(). smt(@BasePoly @ZP.ZModE).
+qed.
+
+
+  lemma peval_X_x cs a : peval (foldr polyM poly1 (map (fun (x : R.t) => polyD2 one (-x)) cs)) a =
+      foldr ( * ) one (map (fun (x : R.t) => a -x) cs).
+  proof.
+    elim cs. simplify. smt(peval_polyC). move => x l ind_hyp. simplify.  rewrite -ind_hyp.
+    rewrite mulpC. rewrite -Xi_polyD2. rewrite -peval_over_Xi. rewrite -peval_add. rewrite peval_X. rewrite -peval_neg. rewrite peval_polyC. smt(@ZP.ZModE).
+  qed.
+ 
+  
   (* Basic facts on Polys not in the standard libary which don't need division *)
   lemma poly0_mul a b : a <> poly0 => b <> poly0 => a * b <> poly0.
    smt(@BasePoly).
   qed.
     
-  op euclidef (m d : sT) (qr : sT * sT) =
+  op euclidef (m d : poly) (qr : poly * poly) =
      m = qr.`1 * d + qr.`2
   /\ (d <> poly0 => 0 <= deg qr.`2 < deg d).
   
-  op edivpoly (m d : sT) =
+  op edivpoly (m d : poly) =
     if d = poly0 then (poly0, m) else choiceb (euclidef m d) (poly0, poly0)
   axiomatized by edivn_def.
 
   (* it would be nice to discharge this axiom *)
-  axiom euclidef_true (m d : sT) : exists x, (euclidef m d) x.
+  axiom euclidef_true (m d : poly) : exists x, (euclidef m d) x.
       
   lemma polyRemThem_corr p d : d <> poly0 =>
     p = ((edivpoly p d).`1 * d) + (edivpoly p d).`2.
@@ -505,7 +498,7 @@ lemma polyM_polyD2 p c1 c0 i : 0 <= i => c1 <> zeror => (p * polyD2 c1 c0).[i + 
   proof.
     smt(@BasePoly polyRemThem_corr).
   qed.
-
+  
     lemma degDiv_2 m d : d <> poly0 => deg (edivpoly m d).`2 < deg d.
   proof.
     move => h. case (exists x, euclidef m d  x). elim.  move => x h'. 
@@ -519,14 +512,14 @@ lemma polyM_polyD2 p c1 c0 i : 0 <= i => c1 <> zeror => (p * polyD2 c1 c0).[i + 
   lemma polyRemThem_r p i :
       polyC (peval p i) = (edivpoly p (X-polyC i)).`2.
   proof.
-    have : peval (edivpoly p (X - polyC i)).`1 i * (i + -i) = zeror. smt(@R). move => h'.     
+    have : peval (edivpoly p (X - polyC i)).`1 i * (i + -i) = zero. smt(@R). move => h'.     
     have : peval p i = peval ((edivpoly p (X - polyC i)).`1 * (X - polyC i) + (edivpoly p (X - polyC i)).`2) i.
     smt(polyRemThem_corr Xi_neq_0). rewrite -peval_add. rewrite -peval_over_Xi. rewrite -peval_add.
     rewrite peval_X. rewrite -peval_neg. rewrite peval_polyC. move => h. rewrite h' in h. rewrite h.
     have : (edivpoly p (X - polyC i)).`2 = polyC (peval (edivpoly p (X - polyC i)).`2 i). rewrite eq_sym. apply polyC_peval.
     smt(degDiv_2 @BasePoly). move => h'''. rewrite h'''. congr.  smt(@R).
   qed. 
-      
+
   lemma ediv_uniq (p a a' b b' d : poly) : d <> poly0 => deg b < deg d => deg b' < deg d =>
     p = a * d + b => p = a' * d + b' => a=a' /\ b=b'.
   proof.    
@@ -590,6 +583,150 @@ lemma polyM_polyD2 p c1 c0 i : 0 <= i => c1 <> zeror => (p * polyD2 c1 c0).[i + 
     have : (- (edivpoly p d).`1) * d - (edivpoly p d).`2 = - ((edivpoly p d).`1 * d + (edivpoly p d).`2).
     smt(@IDPoly). move => h'. rewrite h'. smt(polyRemThem_corr).  
   qed. 
+
+  lemma ediv_mul_qut (a b : poly) : b <> poly0 => (edivpoly (a * b) b).`1 = a.
+  proof.
+    move => h. apply (ediv_uniq_1 (a * b) _ _ (edivpoly (a * b) b).`2 poly0 b); trivial. apply degDiv_2; trivial.
+    smt(@BasePoly). apply polyRemThem_corr; trivial. smt(@BasePoly).
+  qed.
+
+  lemma ediv_mul_rem (a b: poly) : b <> poly0 => (edivpoly (a * b) b).`2 = poly0.
+  proof.
+    move => h. have : (edivpoly (a * b) b).`1 = a /\ (edivpoly (a * b) b).`2 =  poly0.
+    apply (ediv_uniq (a * b) _ _ _ _ b); trivial; trivial. apply degDiv_2; trivial.
+    smt(@BasePoly). apply polyRemThem_corr; trivial. smt(@BasePoly). smt().
+  qed.
+  
+  lemma polyRemThem_1 p i  : (edivpoly p (X-polyC i)).`1 =
+    (edivpoly (p - (edivpoly p (X-polyC i)).`2) (X-polyC i)).`1 + (edivpoly (p - (edivpoly p (X-polyC i)).`2) (X-polyC i)).`2.
+  proof.
+    rewrite polyRemThem_adj. rewrite ediv_mul_qut. apply Xi_neq_0. rewrite ediv_mul_rem. apply Xi_neq_0. smt(@BasePoly).
+  qed.
+
+  lemma edivpoly_quot_poly0 a : (edivpoly poly0 (X - polyC a)).`1 = poly0.
+  proof.
+    case ((edivpoly poly0 (X - polyC a)).`1 = poly0). trivial. move => h.
+    have : poly0 = (edivpoly poly0 (X - polyC a)).`1 * (X - polyC a) + (edivpoly poly0 (X - polyC a)).`2.
+    apply polyRemThem_corr. apply Xi_neq_0. move => j. rewrite -polyRemThem_r in j. smt(@IDPoly @BasePoly).
+qed.
+
+  lemma edivpoly_quot_polyC b a : (edivpoly (polyC b) (X - polyC a)).`1 = poly0.
+  proof.
+    case ((edivpoly (polyC b) (X - polyC a)).`1 = poly0). trivial. move => h.
+    have : polyC b = (edivpoly (polyC b) (X - polyC a)).`1 * (X - polyC a) + (edivpoly (polyC b) (X - polyC a)).`2.
+    apply polyRemThem_corr. apply Xi_neq_0. move => j. rewrite -polyRemThem_r in j. smt(@IDPoly @BasePoly).
+qed.
+
+  lemma poly_eqP_bound (p q : poly) : p = q <=>
+    (deg q <= deg p /\ forall c, 0 <= c < deg p => p.[c] = q.[c]).
+  proof.
+      split => h. rewrite h. trivial.
+      apply poly_eqP. move => x hc. case (x < deg p) => h'. rewrite h. smt(). trivial.
+      rewrite gedeg_coeff. smt(). rewrite gedeg_coeff. smt(). trivial.
+  qed.
+
+  (* The ugliest proof in the world *) (*
+  lemma edivpoly_quot pi a : (edivpoly pi (X - polyC a)).`1 =
+      polyL (mkseq (fun i => foldr Bl.ZP.ZModE.( + ) zero
+        (mkseq (fun (j : int) => pi.[i +1+ j]*exp a j)
+      (deg pi - 1 - i))) (deg pi -1)).
+  proof.
+    (* various small cases *)    
+    case (pi = poly0) => h'. rewrite h'. rewrite edivpoly_quot_poly0. have : deg poly0 = 0. smt(@BasePoly). move => h. rewrite h.
+    have : forall (f : int -> ZP.exp), mkseq f (-1) = []. smt(@List). move => h''. rewrite h''. simplify. smt(@BasePoly).
+    case (exists a, pi = polyC a) => h. elim h. move => a0 h. rewrite h.
+    rewrite edivpoly_quot_polyC. have : forall (f : int -> ZP.exp), mkseq f (deg (polyC a0) - 1) = [].
+    smt(@BasePoly @List). move => g. rewrite g. smt(@BasePoly). have : 2 <= deg pi. smt(@BasePoly). move => g.
+    (* mian case *)
+    apply (ediv_uniq_1 pi  _ _ (edivpoly pi (X - polyC a)).`2 (edivpoly pi (X - polyC a)).`2 (X - polyC a)); trivial.
+    apply Xi_neq_0.   apply degDiv_2; trivial. apply Xi_neq_0. apply degDiv_2; trivial.
+    apply Xi_neq_0. apply polyRemThem_corr; trivial. apply Xi_neq_0.
+    (* We want to prover the polynomials has the expected form *)
+    rewrite -polyRemThem_r. apply poly_eqP_bound. split. have : forall (f : int -> ZP.exp),
+    deg (polyL ( mkseq f (deg pi - 1))) <= deg pi -1. smt(@BasePoly @List). smt(@BasePoly). move => c hc. rewrite polyDE.
+    (* the bottom case *)
+    case (c = 0) => g'. subst. rewrite polyCE. rewrite Xi_polyD2. rewrite polyMD2_0. simplify. rewrite polyLE. simplify.
+    rewrite nth_mkseq. smt(). simplify. rewrite (peval_simp_gen _ _ (deg pi)). trivial. have : deg pi = (deg pi - 1) + 1. smt().
+     move => g''. rewrite g''.  smt(). rewrite mkseqSr. smt(). simplify. have : foldr ZP.ZModE.(+) zero
+   (mkseq (fun (j : int) => pi.[1 + j] * exp a j) (deg pi - 1)) *
+     -a = - (foldr ZP.ZModE.(+) zero (mkseq (fun (j : int) => pi.[1 + j] * exp a j) (deg pi - 1)) * a). smt(@ZP.ZModE.ZModpField).
+     move => g'''. rewrite g'''. rewrite dis_mul_add. smt(@ZP.ZModE). smt(@ZP.ZModE).
+      have: forall (a a' b b' : ZP.ZModE.exp), a = a' => b = b' => a = - b + (a' + b'). smt(@ZP.ZModE). move => h''. apply h''.
+     smt(@ZP.ZModE.ZModpField). congr. smt().  apply (eq_from_nth zero). smt(@List).  move => i hi.
+     rewrite !(nth_map zero). smt(@List). simplify. rewrite !nth_mkseq. smt(@List). smt(@List). 
+     move => @/(\o).  simplify. have : 1 + i = i + 1. smt(). move => w. rewrite w. rewrite exprS. smt(). smt(@ZP.ZModE.ZModpField). 
+    (* resumming *)
+     pose p := c - 1. have : p + 1 <> 0. smt(). simplify. move => w. rewrite Xi_polyD2. have : c = p +1. smt(). 
+   move => l. rewrite l. rewrite polyM_polyD2. smt(). smt(@ZP.ZModE.ZModpField). rewrite polyD2E polyCE. rewrite w.
+     simplify. rewrite !polyLE. simplify. rewrite nth_mkseq. smt().  case (p = deg pi - 2) => g'''.
+     (* top term *)
+     rewrite nth_default. smt(@List). have : deg pi - 1 - p = 1. smt(). move => w''. rewrite w''.  rewrite mkseq1.
+     simplify. have : (pi.[p + 1] * exp a 0 + zero) = pi.[p+1]. smt(@ZP.ZModE.ZModpField). move => h''.
+      smt(@ZP.ZModE.ZModpField).
+     (* last term *)
+     rewrite (nth_mkseq). smt(). simplify. have : deg pi - 1 - p = (deg pi - 2 - p) + 1. smt().
+     move => w''. rewrite w''. rewrite mkseqSr. smt(). simplify. have :  foldr ZP.ZModE.(+) zero
+   (mkseq (fun (j : int) => pi.[p + 2 + j] * exp a j) (deg pi - 1 - (p+1))) * -a =
+     - (foldr ZP.ZModE.(+) zero (mkseq (fun (j : int) => pi.[p + 2 + j] * exp a j) (deg pi - 1 - (p+1)))) * a.
+     smt(@ZP.ZModE.ZModpField). move => w'''. rewrite w'''. rewrite dis_mul_add. smt(@ZP.ZModE). smt(@ZP.ZModE).
+     have: forall (a a' b b' : ZP.ZModE.exp), a = a' => b = b' => a = (a' + b) * oner + - b' + zero. smt(@ZP.ZModE).
+   move => l'. apply l'. smt(@ZP.ZModE.ZModpField). congr.  apply (eq_from_nth zero). smt(@List).  move => i hi.
+     rewrite !(nth_map zero). smt(@List). simplify. rewrite !nth_mkseq. smt(@List).
+     smt(@List). move => @/(\o).  simplify. have : 1 + i = i + 1. smt(). move => s. rewrite s. rewrite exprS. smt(). 
+     smt(@ZP.ZModE.ZModpField). 
+ qed. *)
+
+ (*
+  lemma edivpoly_quot_eval pi a : a <> zero =>  deg pi < GT.order => peval (edivpoly pi (X - polyC a)).`1 a =
+    peval pi a - pi.[0].
+  proof.
+    move => a_neq_0 pi_order.
+    (* poly0 case *)    
+    case (pi = poly0) => h. subst. rewrite edivpoly_quot_poly0. rewrite peval0. smt(@BasePoly @ZP.ZModE).
+    (* polyC case *)
+    case (exists a, pi = polyC a) => h'. elim h' => b h'. subst. rewrite edivpoly_quot_polyC. rewrite !peval_polyC.
+    smt(@BasePoly @ZP.ZModE). rewrite edivpoly_quot. 
+    (* now to try and simplify the top evaluation *) 
+    rewrite (peval_simp_gen _ _ (deg pi -1)).  smt(@BasePoly @List).
+    rewrite (peval_simp_gen _ _ (deg pi)).  smt(@BasePoly @List).
+    have : (mkseq (fun (i : int) => (polyL (mkseq (fun (i0 : int) =>
+    foldr ZP.ZModE.(+) zero  (mkseq (fun (j : int) => pi.[i0 + 1 + j] * exp a j)
+    (deg pi - 1 - i0))) (deg pi - 1))).[i] * exp a i) (deg pi - 1)) =
+    (mkseq (fun (i : int) => foldr ZP.ZModE.(+) zero (mkseq (fun (j : int) => pi.[i + 1 + j] * exp a j)
+          (deg pi - 1 - i)) * exp a i) (deg pi - 1)). apply (eq_from_nth zero). smt(@List). move => i hi. rewrite !nth_mkseq.
+    smt(@List). smt(@List). simplify. rewrite polyLE. simplify. rewrite nth_mkseq. smt(@List). trivial. move => g. rewrite g.
+    have : foldr R.(+) zero (mkseq (fun (i : int) => foldr ZP.ZModE.(+) zero
+          (mkseq (fun (j : int) => pi.[i + 1 + j] * exp a j) (deg pi - 1 - i)) *
+        exp a i) (deg pi - 1)) = foldr R.(+) zero (mkseq
+     (fun (i : int) => foldr ZP.ZModE.(+) zero
+       (mkseq (fun (j : int) => pi.[i + 1 + j] * exp a (j+i)) (deg pi - 1 - i))) (deg pi - 1)).
+         congr. apply (eq_from_nth zero). smt(@List). move => i hi. rewrite !nth_mkseq. smt(@List). smt(@List).
+         simplify. rewrite dis_mul_add. smt(@ZP.ZModE). smt(@ZP.ZModE). congr. apply (eq_from_nth zero). smt(@List).
+   move => j hj. rewrite (nth_map zero). smt(@List). rewrite !nth_mkseq. smt(@List). smt(@List). simplify.
+          rewrite exprD. smt(@ZP.ZModE.ZModpField). smt(@ZP.ZModE.ZModpField). move => g'. rewrite g'.
+      pose f := (fun l => pi.[l+1] * exp a l). have : (mkseq (fun (i : int) => foldr ZP.ZModE.(+) zero
+          (mkseq (fun (j : int) => pi.[i + 1 + j] * exp a (j + i))
+            (deg pi - 1 - i))) (deg pi - 1)) = mkseq (fun i => foldr ZP.ZModE.(+) zero (mkseq (fun (j :int) => f (i + j)) (deg pi -1-i))) (deg pi - 1). apply (eq_from_nth zero). smt(@List). move => i hi. rewrite !nth_mkseq. smt(@List). smt(@List).
+     simplify. congr. apply (eq_from_nth zero). smt(@List). move => i0 hi0 @/f. smt(@List).  
+      move => g''. rewrite g''. have : R.(+) = ZP.ZModE.(+). smt(). move => l. rewrite l.
+              pose expa := (fun (x : ZP.exp) (i : int) => foldr ZP.ZModE.(+) zero (mkseq (fun y => x) i)).
+              rewrite (double_loop_rearr f ZP.ZModE.(+) zero expa). move => a0 i hi @/expa. rewrite mkseqSr.
+    trivial. simplify. congr. congr. apply (eq_from_nth zero). smt(@List). move => j hj. rewrite !nth_mkseq. smt(@List).
+              smt(@List). trivial. move => a0 i hi @/expa. subst. rewrite mkseq1. simplify. smt(@ZP.ZModE).
+              move => a0 @/expa. rewrite mkseq0. trivial. smt(@ZP.ZModE). smt(@ZP.ZModE).
+    smt(@ZP.ZModE). smt(@BasePoly). clear g g' g''. move => @/f @/expa.   trivial. pose c := deg pi -1.
+    have : deg pi = c + 1. smt(). move => g. rewrite g. rewrite mkseqSr. smt(@BasePoly). simplify.
+    have : forall (a a' b b' : ZP.exp), a = a' => b =b' => a = b + a' - b'. smt(@ZP.ZModE).
+      move => g'. apply g'. move => @/(\o). simplify. congr. apply (eq_from_nth zero). smt(@List). move => i hi.
+              rewrite !nth_mkseq. smt(@List). smt(@List). simplify.
+    (* Need to figure out how to simplify the top *)
+              have : forall j, 0 <= j => j + 1 < Bl.GT.order =>
+              foldr ZP.ZModE.(+) zero (mkseq (fun (_ : int) => pi.[i + 1] * exp a i) (j + 1)) =
+      (ZP.ZModE.inzmod (j+1)) * pi.[i + 1] * exp a (i). apply intind. simplify. rewrite mkseq1. simplify.  smt(@ZP.ZModE).
+     simplify.  move => i0 hi0 ind_hyp i0_order. have : i0 + 2 =  i0 + 1 + 1. smt(). move => l'. rewrite l'. rewrite mkseqS. smt().
+     rewrite foldr_rcons. smt(@ZP.ZModE). smt(@ZP.ZModE). simplify. rewrite ind_hyp. smt(). admit.  
+       move => g''. rewrite g''. smt(). smt(@List). admit.  move => g''. rewrite g''. smt(). rewrite exprM.          
+  qed. *)
   
   lemma degDiv m d : deg (edivpoly m d).`1 <= deg m.
   proof.
@@ -617,12 +754,13 @@ qed.
     smt(@BasePoly).
   qed.
 
+  
   (* p/(X-i)[a] = (p[a]-p[i])/(a-i) *)
-  lemma prt_eval p (i a : GP.exp) :  (-i) + a <> zeror =>
+  lemma prt_eval p (i a : ZP.exp) :  (-i) + a <> zero =>
     peval (edivpoly p (X - polyC i)).`1 a = (peval p a - peval p i)/(a-i).
       move => g. have : peval (edivpoly p (X - polyC i)).`1 a * (a-i) =  (peval p a - peval p i) =>
       peval (edivpoly p (X - polyC i)).`1 a = ((peval p a - peval p i) / (a - i))%R.
-      move => h. rewrite -h. rewrite -R.mulrA. rewrite R.mulrV. smt(@GP.ZModE).  smt(@GP.ZModE).
+      move => h. rewrite -h. rewrite -R.mulrA. rewrite R.mulrV. smt(@ZP.ZModE).  smt(@ZP.ZModE).
       move => h. apply h. have : (a-i) = peval (X - polyC i) a.
       rewrite -peval_add. rewrite -peval_neg.
       rewrite peval_polyC. rewrite peval_X. trivial. move => h'. rewrite h'. rewrite peval_over_Xi.
@@ -631,31 +769,31 @@ qed.
     qed.
 
     
-  lemma prt_eval2 phi phi' (i a b : GP.exp) : (-i) + a <> zeror =>
+  lemma prt_eval2 phi phi' (i a b : ZP.exp) : (-i) + a <> zero =>
       peval (edivpoly phi (X - polyC i)).`1 a + b * peval (edivpoly phi' (X - polyC i)).`1 a =
       peval (edivpoly (b ** phi' + phi) (X - polyC i)).`1 a.
   proof.
     move => h. rewrite !prt_eval; trivial. rewrite -!peval_add -!peval_mul.
     have : peval phi' a * b + peval phi a - (peval phi' i * b + peval phi i) =
-    b * (peval phi' a - peval phi' i) + peval phi a - peval phi i. rewrite GP.ZModE.ZModpField.opprD.
-    rewrite !GP.ZModE.ZModpField.addrA. congr; trivial. rewrite GP.ZModE.ZModpField.addrC.
-    rewrite GP.ZModE.ZModpField.addrA.
-    pose x := peval phi' a. pose y := peval phi' i. smt(@GP.ZModE).
+    b * (peval phi' a - peval phi' i) + peval phi a - peval phi i. rewrite ZP.ZModE.ZModpField.opprD.
+    rewrite !ZP.ZModE.ZModpField.addrA. congr; trivial. rewrite ZP.ZModE.ZModpField.addrC.
+    rewrite ZP.ZModE.ZModpField.addrA.
+    pose x := peval phi' a. pose y := peval phi' i. smt(@ZP.ZModE).
 
-    move => g. rewrite g. rewrite !GP.ZModE.ZModpField.mulrDl. rewrite -GP.ZModE.ZModpField.addrA.
-    rewrite (GP.ZModE.ZModpField.addrC). rewrite -GP.ZModE.ZModpField.mulrDl. smt(@GP.ZModE). 
+    move => g. rewrite g. rewrite !ZP.ZModE.ZModpField.mulrDl. rewrite -ZP.ZModE.ZModpField.addrA.
+    rewrite (ZP.ZModE.ZModpField.addrC). rewrite -ZP.ZModE.ZModpField.mulrDl. smt(@ZP.ZModE). 
 qed.
 
 
-lemma Xi_eval_inv i : GP.ZModE.inv (peval (X - polyC i) i) = peval (X - polyC i) i.
+lemma Xi_eval_inv i : ZP.ZModE.inv (peval (X - polyC i) i) = peval (X - polyC i) i.
 proof.
-  rewrite !Xi_eval. smt(@GP.ZModE).
+  rewrite !Xi_eval. smt(@ZP.ZModE).
 qed.
 
 (* the number of roots is bounded by the degree - 1 *)
 (* Note that in easycrypt libary x has degree 2 and x^2 has degree 3 *)
 axiom roots_bounded_by_degree p rs : p <> poly0 => uniq rs => all (BasePoly.root p) rs => size rs <= deg p -1.
-op findroots : poly -> GP.exp list.
+op findroots : poly -> ZP.exp list.
 axiom findroots_corr p rs : rs = findroots p => uniq rs /\  all (BasePoly.root p) rs.
 axiom findroots_size p : 1 < deg p => size (findroots p) = deg p -1.
 
@@ -681,66 +819,66 @@ qed.
 
 (* Some lemmas for polynomial  *)
 
-op lb (j : GP.exp)(js: GP.exp list) : poly = foldr polyM poly1 (map (fun (x : GP.exp) => (polyD2 (invr (j-x)) ((-x)/(j-x)))) js).
+op lb (j : ZP.exp)(js: ZP.exp list) : poly = foldr polyM poly1 (map (fun (x : ZP.exp) => (polyD2 (inv (j-x)) ((-x)/(j-x)))) js).
 
 lemma deg_lb j js : deg (lb j js) <= size js + 1.
  proof.
  move => @/lb. elim js. simplify. smt(@BasePoly). move => x l ind_hyp. simplify.
- have : deg (polyD2 (invr (j - x)) ((-x) / (j - x))) <= 2. apply deg_leq_polyD2. smt(@BasePoly).
+ have : deg (polyD2 (inv (j - x)) ((-x) / (j - x))) <= 2. apply deg_leq_polyD2. smt(@BasePoly).
 qed.
 
-lemma lb_1 js i : 0 <= i < size js => uniq js => peval (lb (nth zeror js i) (rem (nth zeror js i) js)) (nth zeror js i) = oner.
+lemma lb_1 js i : 0 <= i < size js => uniq js => peval (lb (nth zero js i) (rem (nth zero js i) js)) (nth zero js i) = one.
 proof.
-  move => h h' @/lb. rewrite peval_polyD2_prod.  apply foldr_id; trivial. smt(@R).  apply (all_nthP _ _ oner). move => i0 hi0.
-  rewrite !size_map in hi0. rewrite size_rem in hi0. smt(@List). rewrite (nth_map (oner,oner)). smt(@List).
-  rewrite (nth_map zeror). smt(@List). simplify. have : (nth zeror js i - nth zeror (rem (nth zeror js i) js) i0) <> zeror.
-  have : forall (a b : GP.exp), a <> b => a - b <> zeror. smt(@GP.ZModE.ZModpField). move => g. apply g. smt(@List).
-   smt(@GP.ZModE.ZModpField).
+  move => h h' @/lb. rewrite peval_polyD2_prod.  apply foldr_id; trivial. smt(@R).  apply (all_nthP _ _ one). move => i0 hi0.
+  rewrite !size_map in hi0. rewrite size_rem in hi0. smt(@List). rewrite (nth_map (one,one)). smt(@List).
+  rewrite (nth_map zero). smt(@List). simplify. have : (nth zero js i - nth zero (rem (nth zero js i) js) i0) <> zero.
+  have : forall (a b : ZP.exp), a <> b => a - b <> zero. smt(@ZP.ZModE.ZModpField). move => g. apply g. smt(@List).
+   smt(@ZP.ZModE.ZModpField).
 qed.
 
 lemma lb_0 js (i i0 : int) : i<> i0 => 0 <= i0 < size js => 0 <= i < size js => uniq js => 
-    peval (lb (nth zeror js i0) (rem (nth zeror js i0) js)) (nth zeror js i) = zeror.
+    peval (lb (nth zero js i0) (rem (nth zero js i0) js)) (nth zero js i) = zero.
 proof.
-  move => h h' h'' h'''. rewrite peval_polyD2_prod. apply foldr_ann_in. smt(@R). smt(@R). apply (nthP zeror).
-  exists (if i < index (nth zeror js i0) js then i else i -1).
-  have : index (nth zeror js i0) js <> i. smt(@List). move => g.
+  move => h h' h'' h'''. rewrite peval_polyD2_prod. apply foldr_ann_in. smt(@R). smt(@R). apply (nthP zero).
+  exists (if i < index (nth zero js i0) js then i else i -1).
+  have : index (nth zero js i0) js <> i. smt(@List). move => g.
   (* size *)
   split. rewrite !size_map. rewrite size_rem. smt(@List). smt(@List). 
   (* eq *)
-  rewrite (nth_map (zeror, zeror)). smt(@List). rewrite (nth_map (zeror)). smt(@List). rewrite rem_nth. smt(@List).
-  simplify. case(i < index (nth zeror js i0) js) => g'. rewrite g'.  simplify. smt(@R).
-  have : ! i - 1 < index (nth zeror js i0) js. smt(@List).  move => g''. rewrite g''. smt(@R).
+  rewrite (nth_map (zero, zero)). smt(@List). rewrite (nth_map (zero)). smt(@List). rewrite rem_nth. smt(@List).
+  simplify. case(i < index (nth zero js i0) js) => g'. rewrite g'.  simplify. smt(@R).
+  have : ! i - 1 < index (nth zero js i0) js. smt(@List).  move => g''. rewrite g''. smt(@R).
 qed.
 
-op lbs (js: GP.exp list) : poly list  = mkseq (fun i => lb (nth zeror js i) (rem (nth zeror js i)  js)) (size js).
+op lbs (js: ZP.exp list) : poly list  = mkseq (fun i => lb (nth zero js i) (rem (nth zero js i)  js)) (size js).
 
-op interpolate (js: GP.exp list)(phiis : GP.exp list) : poly = foldr polyD poly0
-                              (map (fun (x : GP.exp*poly) => x.`1 ** x.`2) (zip phiis (lbs js))).
+op interpolate (js: ZP.exp list)(phiis : ZP.exp list) : poly = foldr polyD poly0
+                              (map (fun (x : ZP.exp*poly) => x.`1 ** x.`2) (zip phiis (lbs js))).
 
 lemma interpolate_deg js phiis: size js = size phiis =>  deg (interpolate js phiis) <= size js.
   move => h @/interpolate.
   have : forall a, all (fun x => deg x <= size js) a => deg (foldr BasePoly.(+) poly0 a) <= size js.
   move => a. elim a. smt(@BasePoly). smt(@BasePoly). move => g. apply g. apply (all_nth _ poly0). move => i hi.  
-  rewrite (nth_map (zeror, poly0)). smt(@List). simplify. rewrite nth_zip. smt(@List). simplify. apply degZ_le_gen.
+  rewrite (nth_map (zero, poly0)). smt(@List). simplify. rewrite nth_zip. smt(@List). simplify. apply degZ_le_gen.
   rewrite nth_mkseq. smt(@List). simplify. smt(deg_lb @List). 
  qed.
   
 (* prove interpolation *)                              
 lemma interpolate_int js phis : size js = size phis => uniq js => map (fun x => peval (interpolate js phis) x) js = phis.
 proof.
-  move => h uniq. apply (eq_from_nth zeror). rewrite size_map; trivial. rewrite size_map; trivial.  move => i hi.
-  rewrite (nth_map zeror). trivial. simplify. move => @/interpolate. rewrite peval_sum. 
-  have : (map (fun (phi : poly) => peval phi (nth zeror js i)) (map (fun (x : GP.exp * poly) => x.`1 ** x.`2) (zip phis (lbs js))))
-= mkseq (fun i0 => peval (nth zeror phis i0 ** (lb (nth zeror js i0) (rem (nth zeror js i0) js))) (nth zeror js i)) (size js).
+  move => h uniq. apply (eq_from_nth zero). rewrite size_map; trivial. rewrite size_map; trivial.  move => i hi.
+  rewrite (nth_map zero). trivial. simplify. move => @/interpolate. rewrite peval_sum. 
+  have : (map (fun (phi : poly) => peval phi (nth zero js i)) (map (fun (x : ZP.exp * poly) => x.`1 ** x.`2) (zip phis (lbs js))))
+= mkseq (fun i0 => peval (nth zero phis i0 ** (lb (nth zero js i0) (rem (nth zero js i0) js))) (nth zero js i)) (size js).
   (* rewrite as mkseq *)
-  apply (eq_from_nth zeror).  smt(@List). move => i0 hi0. rewrite (nth_map poly0). smt(@List). rewrite (nth_map (zeror, poly0)).
+  apply (eq_from_nth zero).  smt(@List). move => i0 hi0. rewrite (nth_map poly0). smt(@List). rewrite (nth_map (zero, poly0)).
   smt(@List). rewrite nth_mkseq. smt(@List). smt(@List). 
   (* resume main *)
   move=> g. rewrite g. rewrite (foldr_id_nth_mkseq _ _ _  i); trivial. smt(@R). smt(@R). smt(@R).
   (* all basis except i have roots at *)
-  apply (all_nthP _ _ zeror). move => i0 hi0. rewrite size_mkseq in hi0. rewrite nth_mkseq. smt(). simplify.
+  apply (all_nthP _ _ zero). move => i0 hi0. rewrite size_mkseq in hi0. rewrite nth_mkseq. smt(). simplify.
   rewrite -peval_mul. rewrite lb_0; trivial. smt(). smt(@List). smt(@R).
-  apply (all_nthP _ _ zeror). move => i0 hi0. rewrite size_mkseq in hi0. rewrite nth_mkseq. smt(). simplify.
+  apply (all_nthP _ _ zero). move => i0 hi0. rewrite size_mkseq in hi0. rewrite nth_mkseq. smt(). simplify.
   rewrite -peval_mul. rewrite lb_0; trivial. smt(). smt(@List). smt(@R). 
   (* 1 everywhere else *)
   simplify. rewrite -peval_mul. rewrite lb_1; trivial. smt(@R).
@@ -752,7 +890,7 @@ lemma interpolate_uniq js phis pi pi' : deg pi <= size js => deg pi' <= size js 
 proof.
   move => deg1 deg2 uniq_js eval1 eval2. case(pi = pi') => h. trivial.
   have: size js <= deg (pi-pi') - 1. apply roots_bounded_by_degree; trivial. smt(@IDPoly).
-  apply (all_nth _ zeror). move => i hi @/root. simplify. rewrite -peval_add. rewrite -peval_neg. smt(@R @List).
+  apply (all_nth _ zero). move => i hi @/root. simplify. rewrite -peval_add. rewrite -peval_neg. smt(@R @List).
   smt(@BasePoly).
 qed.
 
@@ -768,12 +906,12 @@ proof.
 qed.
  
 lemma interpolate_nth js phiis i : size js = size phiis =>
-    (interpolate js phiis).[i] = foldr R.( + ) zeror
-    (map (fun (x : GP.exp*GP.exp) => x.`1 * (lb x.`2 (rem x.`2  js)).[i]) (zip phiis js)).
+    (interpolate js phiis).[i] = foldr R.( + ) zero
+    (map (fun (x : ZP.exp*ZP.exp) => x.`1 * (lb x.`2 (rem x.`2  js)).[i]) (zip phiis js)).
 proof.
-  move => h @/interpolate. rewrite poly_sum_nth. congr.  apply (eq_from_nth zeror). smt(@List).
-  move => i0 hi0. rewrite (nth_map poly0). smt(@List). rewrite (nth_map (zeror,zeror)). smt(@List).
-  rewrite (nth_map (zeror,poly0)). smt(@List). simplify. rewrite nth_zip. smt(@List).
+  move => h @/interpolate. rewrite poly_sum_nth. congr.  apply (eq_from_nth zero). smt(@List).
+  move => i0 hi0. rewrite (nth_map poly0). smt(@List). rewrite (nth_map (zero,zero)). smt(@List).
+  rewrite (nth_map (zero,poly0)). smt(@List). simplify. rewrite nth_zip. smt(@List).
    rewrite nth_zip. smt(@List). simplify. rewrite nth_mkseq. smt(@List). simplify. smt(@BasePoly).
 qed.
 
@@ -817,9 +955,9 @@ proof.
   rewrite pairwise_add_nth. rewrite pairwise_sum_size. trivial. smt(@List). smt(@List). smt(@List). trivial.
 qed.
 
-op interpolate_exp (js : GP.exp list)(phiis : GB.group list) : GB.group list =
+op interpolate_exp (js : ZP.exp list)(phiis : GB.group list) : GB.group list =
 foldr pairwise_add (mkseq (fun (x :int) => GB.e) (size js))
-(map (fun (x : GB.group*poly) => mkseq (fun i => GB.( ^ ) x.`1 (GP.ZModE.asint x.`2.[i])) (size js)) (zip phiis (lbs js))).
+(map (fun (x : GB.group*poly) => mkseq (fun i => GB.( ^ ) x.`1 (ZP.ZModE.asint x.`2.[i])) (size js)) (zip phiis (lbs js))).
 
 lemma interpolate_exp_size js phiis : size (interpolate_exp js phiis) = size js.
 proof.
@@ -833,22 +971,23 @@ qed.
     
 op peval_exp g_phi a =  List.foldr GB.( * ) GB.e
       (mkseq (fun (i : int) => GB.( ^ )(nth GB.e g_phi i)
-          (GP.ZModE.asint (GP.ZModE.exp a i))) (size g_phi)).
+          (ZP.ZModE.asint (ZP.ZModE.exp a i))) (size g_phi)).
 
+(*
 lemma inter_eval js phiis a : size phiis = size js =>
-  peval_exp (interpolate_exp js (map (fun x1 => GB.(^) GB.g (GP.ZModE.asint x1)) phiis)) a =
-    GB.( ^ ) GB.g (GP.ZModE.asint (peval (interpolate js phiis) a)).
+  peval_exp (interpolate_exp js (map (fun x1 => GB.(^) GB.g (ZP.ZModE.asint x1)) phiis)) a =
+    GB.( ^ ) GB.g (ZP.ZModE.asint (peval (interpolate js phiis) a)).
 proof.
   move => h @/peval_exp. rewrite interpolate_exp_size. rewrite (peval_simp_gen _  _ (size js)). apply interpolate_deg; trivial.
-  rewrite h. trivial. rewrite -(prod_sum_eq _ zeror). move => @/interpolate_exp. congr. apply (eq_from_nth GB.e).
+  rewrite h. trivial. rewrite -(prod_sum_eq _ zero). move => @/interpolate_exp. congr. apply (eq_from_nth GB.e).
   smt(@List). move => i hi. rewrite size_mkseq in hi. rewrite !nth_mkseq. smt(). smt(@List). simplify. 
   rewrite (pairwise_sum_nth (size js) _ i).  apply (all_nth _ []). move => i0 hi0. simplify. rewrite (nth_map (GB.e,poly0)).
   smt(@List). smt(@List). rewrite nth_mkseq. smt(). simplify. rewrite -exp_GB_asint_mul. rewrite GB.expM. congr.
   (* go it to the point where neec only show that the coefficents are equal *)
-  rewrite interpolate_nth. rewrite h. trivial. rewrite -(prod_sum_eq _ zeror). congr. apply (eq_from_nth GB.e).
+  rewrite interpolate_nth. rewrite h. trivial. rewrite -(prod_sum_eq _ zero). congr. apply (eq_from_nth GB.e).
   smt(@List). move => i0 hi0. rewrite (nth_map []). smt(@List). rewrite nth_mkseq. smt(@List). simplify.
-  rewrite (nth_map (zeror,zeror)). smt(@List). rewrite (nth_map (GB.e,poly0)). smt(@List). simplify.
-  rewrite nth_mkseq. smt(@List). simplify. rewrite nth_zip. smt(@List). simplify. rewrite (nth_map zeror). smt(@List).
+  rewrite (nth_map (zero,zero)). smt(@List). rewrite (nth_map (GB.e,poly0)). smt(@List). simplify.
+  rewrite nth_mkseq. smt(@List). simplify. rewrite nth_zip. smt(@List). simplify. rewrite (nth_map zero). smt(@List).
   simplify. rewrite -GB.expM. rewrite exp_GB_asint_mul. congr. congr. rewrite nth_zip. smt(@List). simplify.
   rewrite nth_mkseq. smt(@List). trivial. trivial.
 qed.
@@ -871,14 +1010,14 @@ lemma interpolate_corr2_tail j js phi phis :  uniq (j :: js) => size js = size p
 qed.
 
 lemma interpolate_corr2_nth js phis j :  uniq js => size js = size phis =>0 <= j && j < size js =>
-    peval (interpolate js phis) (nth GP.ZModE.zero js j) = nth GP.ZModE.zero phis j.
+    peval (interpolate js phis) (nth ZP.ZModE.zero js j) = nth ZP.ZModE.zero phis j.
 proof.
   move => g g' h. have : map (fun x => peval (interpolate js phis) x) js = phis. apply interpolate_corr2; trivial. move => h'.
-  pose phi :=  (interpolate js phis). rewrite -h'. rewrite (nth_map GP.ZModE.zero).  trivial. simplify.  trivial.
+  pose phi :=  (interpolate js phis). rewrite -h'. rewrite (nth_map ZP.ZModE.zero).  trivial. simplify.  trivial.
 qed.
 
 lemma interpolate_corr2_nth_tail j js phi phis i :  uniq (j :: js) => size js = size phis => 0 <= i && i < size js =>
-    peval (interpolate (j :: js) (phi :: phis)) (nth GP.ZModE.zero js i) = nth GP.ZModE.zero phis i.
+    peval (interpolate (j :: js) (phi :: phis)) (nth ZP.ZModE.zero js i) = nth ZP.ZModE.zero phis i.
 proof.
    move => g g' h. have : map (fun x => peval (interpolate (j :: js) (phi :: phis)) x) js = phis.
   apply interpolate_corr2_tail; trivial. smt(@List).
@@ -891,6 +1030,15 @@ proof.
   move => h0 h1 h2. apply interpolate_corr; trivial. smt(interpolate_deg). smt(@List).
 qed.
 
+lemma inter_inter_gen js js' phi phi' : size js' = size phi' => size js = size js' =>
+    uniq js =>
+    phi = map (peval (interpolate js' phi')) js =>
+    interpolate js phi =
+    interpolate js' phi'.
+proof.
+  move => h0 h1 h2 h. rewrite h. apply interpolate_corr; trivial. smt(interpolate_deg). smt(@List).
+qed.
+
 lemma inter_inter_tail a x js js'0 phi : size js'0 = size phi => size js = size phi =>
     uniq (a :: js) => uniq (a :: js'0) =>
     interpolate (a :: js) (x :: map (peval (interpolate (a :: js'0) (x :: phi))) js) =
@@ -900,7 +1048,7 @@ lemma inter_inter_tail a x js js'0 phi : size js'0 = size phi => size js = size 
  qed.
 
 (* randomly sampling the coefficents of a polynomial or sampling eval values is the same *)
-lemma interpolate_prob (phiis : GP.exp * GP.exp list) js t : uniq js => size js = t => size phiis.`2 = t -1 =>
+lemma interpolate_prob (phiis : ZP.exp * ZP.exp list) js t : uniq js => size js = t => size phiis.`2 = t -1 =>
   mu1 (FD.dt `*` dlist FD.dt (t - 1)) phiis =
 mu1 (dpoly t FD.dt)
     (interpolate js (phiis.`1 :: phiis.`2)).    
@@ -909,48 +1057,48 @@ proof.
   smt(@List). smt(@FD). rewrite (in_dmap1E_can _ _ (fun pi => mkseq (fun i => pi.[i]) t)). move => @/polyL.
   apply poly_eqP. move => c hc. rewrite coeffE. smt(@BasePoly). move =>  @/prepolyL. simplify.
   case (c < deg (interpolate js (phiis.`1 :: phiis.`2))). move => g. rewrite nth_mkseq. smt(interpolate_deg). trivial.
-  smt(@List @BasePoly). move => y hy heq. simplify. rewrite -heq. apply (eq_from_nth zeror). smt(@List @DList).
+  smt(@List @BasePoly). move => y hy heq. simplify. rewrite -heq. apply (eq_from_nth zero). smt(@List @DList).
   move => i hi. rewrite nth_mkseq. smt(@List @DList). smt(@List @BasePoly).
   rewrite (AddDistr.dlist_mu1  _ _ GT.order). smt(@List). smt(@FD). trivial.
 qed.
 
 (* You can't do better then guessing an evaluation if the polynomial is random up to deg-1 indepedent points *)
-axiom interpolate_prob2 phii i (v2 : GP.exp list) v3 : !(i \in v2) => size v2 = t-1 =>
-  mu FD.dt (fun (x : GP.exp) => mu FD.dt (fun (x0 : GP.exp) =>
+axiom interpolate_prob2 phii i (v2 : ZP.exp list) v3 : !(i \in v2) => size v2 = t-1 =>
+  mu FD.dt (fun (x : ZP.exp) => mu FD.dt (fun (x0 : ZP.exp) =>
     phii = peval (interpolate (x :: v2) (x0 :: v3)) i) = inv GB.order%r) = 1%r.
 
 (* this should follow from interpolate_prob *)
 axiom interpolate_prob3 phi j js : mu1 (dpoly Bl.t FD.dt) phi =
 mu1 (dlet FD.dt (fun x0 => dmap (dlist FD.dt (Bl.t - 1))
-  (fun (phiis'0 : GP.exp list) => (x0, phiis'0)))) (peval phi j, map (peval phi) js).
+  (fun (phiis'0 : ZP.exp list) => (x0, phiis'0)))) (peval phi j, map (peval phi) js).
 
 
-axiom  interpolate_prob2_dcond phii i (v2 : GP.exp list) v3 : !(i \in v2) => size v2 = t-1 =>
-  mu (dcond Bl.FD.dt (fun (x : Bl.GP.exp) => ! (x \in v2)))
-  (fun (x : GP.exp) => mu Bl.FD.dt (fun (x0 : GP.exp) =>
+axiom  interpolate_prob2_dcond phii i (v2 : ZP.exp list) v3 : !(i \in v2) => size v2 = t-1 =>
+  mu (dcond Bl.FD.dt (fun (x : Bl.ZP.exp) => ! (x \in v2)))
+  (fun (x : ZP.exp) => mu Bl.FD.dt (fun (x0 : ZP.exp) =>
   phii = peval (interpolate (x :: v2) (x0 :: v3)) i) = inv Bl.GB.order%r) = 1%r.
 
 lemma interpolate_in_dpoly js phis t : size js = t => size phis = t =>
     interpolate js phis \in dpoly t FD.dt.
 proof.
 move => h0 h1. rewrite supp_dpoly. smt(@List). split. rewrite -h0. apply interpolate_deg; trivial. smt(). smt(@Poly @FD).
-qed.
+qed.*)
 
 (* factor find - Given a non-zero polynomial with a root at i *)
 (* and a Tsdh instance with secrect i returns i *)
-op factorFind (p : poly)(ga : Bl.GB.group list): GP.exp =
-  nth zeror (findroots p) (find (fun x=> ga = Bl.mkKey x) (findroots p)).
+op factorFind (p : poly)(ga : Bl.GB.group list): ZP.exp =
+  nth zero (findroots p) (find (fun x=> ga = Bl.mkKey x) (findroots p)).
 
 lemma factorFindCorr p p' a : p <> p' =>
   peval p a = peval p' a =>
    factorFind (p - p') (mkKey a) = a.
 proof.
   move => h h'. case (deg (p-p') = 1) => g. have : exists a, (p-p') = polyC a. smt(@BasePoly). move => a0. elim a0.
-  move => a0 g'. have : a0 <> zeror. smt(@BasePoly). move => h''. have : peval (p - p') a = zeror.
-  rewrite -peval_add -peval_neg. smt(@GP.ZModE). move => g''. rewrite g' in g''. rewrite peval_polyC in g''. trivial.
+  move => a0 g'. have : a0 <> zero. smt(@BasePoly). move => h''. have : peval (p - p') a = zero.
+  rewrite -peval_add -peval_neg. smt(@ZP.ZModE). move => g''. rewrite g' in g''. rewrite peval_polyC in g''. trivial.
   have : a \in (findroots (p-p')). apply root_in_findroots. smt(@BasePoly). rewrite -peval_add. rewrite -peval_neg.
-  smt(@GP.ZModE). move => g' @/factorFind. pose pre := (fun (x : GP.ZModE.exp) => mkKey a = mkKey x).
-  have : pre (nth zeror (findroots (p - p')) (find pre (findroots (p - p')))). apply nth_find. apply hasP.
+  smt(@ZP.ZModE). move => g' @/factorFind. pose pre := (fun (x : ZP.ZModE.exp) => mkKey a = mkKey x).
+  have : pre (nth zero (findroots (p - p')) (find pre (findroots (p - p')))). apply nth_find. apply hasP.
   exists a. trivial. move => h''. apply mkKeyBij. smt().
 qed.
 
