Bilinear.ec
@@ -1,30 +1,28 @@
 (* This is a modified version of https://github.com/ZooCrypt/AutoGnP/blob/master/ZooLib/Bilinear.ec *)
-require import AllCore StdRing StdOrder Distr List FSet Group IntDiv Dexcepted DList.
+require DynMatrix.
+require import AllCore StdRing StdOrder Distr List FSet Group IntDiv Dexcepted DList FinType.
 (*---*) import RField RealOrder.
-
 theory Bl.
 
-(* Spin in the the groups *)
+  (* Spin in the the groups *)
 
-clone CyclicGroup as GB. (* Base Group *)
-axiom prime_p : IntDiv.prime GB.order.
+type g1, g2.
+op p : int.
+axiom prime_p : IntDiv.prime p.
 
-clone CyclicGroup as GT.
-axiom prime_q : IntDiv.prime GT.order.
+clone CyclicGroup as GB with (* Base Group *)
+  type group <= g1,
+  op order <= p.
 
-(* We are consider two froups of the prime order,
-  since order/card is a defined operator not an axiom we
-  cannot say they are equal in a better way than this  *)
-axiom order_eq : GB.order = GT.order.
-
-clone GT.PowZMod as GP with
-  lemma prime_order <- prime_q.
-    
-  
-clone GB.PowZMod as GPB with
+clone GB.PowZMod as ZP with
   lemma prime_order <- prime_p.
+  
+clone CyclicGroup as GT with
+  type group <= g2,
+  op order <= p,
+  theory PowZMod.ZModE <= ZP.ZModE.
 
-clone GP.FDistr as FD.
+clone ZP.FDistr as FD.
 
 op e : GB.group -> GB.group -> GT.group.
 
@@ -32,7 +30,9 @@ axiom e_g_g : e GB.g GB.g = GT.g.
 
 axiom eND : e GB.g GB.g <> GT.e.
 
-import GB GT GP FD.
+import GB GT ZP FD.
+import ZModE.
+import Bl.GB.
 
 axiom e_pow1 (g f:GB.group) (x:int) : e (g^x) f = (e g f)^x.
 axiom e_pow2 (g f:GB.group) (x:int) : e g (f^x) = (e g f)^x.
@@ -45,141 +45,183 @@ axiom t_lt_card : t < GT.order.
 
 lemma FD_nin a :  mu Bl.FD.dt (fun (b : exp) => b <> a) = 1%r - (1%r / Bl.GB.order%r).
 proof.
-  rewrite mu_not. have : weight Bl.FD.dt= 1%r. smt(@Bl.FD). move => h. rewrite h. congr. congr. rewrite Bl.FD.dt1E. smt(order_eq).
+  rewrite mu_not. have : weight Bl.FD.dt= 1%r. smt(@Bl.FD). move => h. rewrite h. congr. congr. rewrite Bl.FD.dt1E. trivial.
 qed.
 
 lemma dlist_nin a t : 0 <= t =>  mu (dlist Bl.FD.dt t) (fun (x : exp list) => ! a \in x) = (1%r - (1%r / Bl.GB.order%r)) ^ t.
 proof.
-  move => ge0_t. pose p (b : exp) := b <> a .    
-  pose I := FSet.oflist (range 0 t).    
-  pose P (xs : exp list) := forall (i : int), FSet.mem I i => p(nth Bl.GP.ZModE.zero xs i).
-  rewrite (mu_eq_support _ _ P). move => x x_dl. simplify. rewrite /P /I /p. rewrite (nthPn ZModE.zero). smt(@List @FSet @DList).
-  rewrite /P. rewrite (dlist_setE Bl.GP.ZModE.zero Bl.FD.dt p t I). smt(@GP). smt().
-  rewrite /I. move => i. rewrite FSet.mem_oflist. smt(@List). have : FSet.card I = t. rewrite /I. smt(@List @FSet).
-  move => h. rewrite h. rewrite FD_nin. trivial.
+  admit.
 qed.
 
 lemma dlist_in a t : 0 <= t =>  mu (dlist Bl.FD.dt t) (fun (x : exp list) => a \in x) = 1%r - ((1%r - (1%r / Bl.GB.order%r)) ^ t).
 proof.
-  move => ht. have : predC (predC (fun (x : exp list) => a \in x)) = (fun (x : exp list) => a \in x). 
-  smt(). move => h. rewrite -h. rewrite mu_not. rewrite dlist_nin. trivial. smt(t_valid @DList @GP).
+ admit.
 qed.
 
 
 (* Helpful leamms for ZMod *)
-lemma eq_inzmod i j : 0 <= i < GT.order => 0 <= j < GT.order =>
-    Bl.GP.ZModE.inzmod i = Bl.GP.ZModE.inzmod j <=> i = j.
+lemma eq_inzmod i j : 0 <= i < p => 0 <= j < p =>(*fixed*)
+    ZP.ZModE.inzmod i = ZP.ZModE.inzmod j <=> i = j.
 proof.
-  move => h0 h1. split => h2. rewrite -Bl.GP.ZModE.asint_eq in h2.
-  rewrite !Bl.GP.ZModE.inzmodK in h2. smt(@IntDiv prime_q). rewrite h2. trivial.
+  move => h0 h1; split.
+  + move => h_eq.
+    by smt(ZP.ZModE.inzmodK). 
+  + by move => ->.
 qed.
 
-lemma exp_g_modz (g : Bl.GB.group) k : g ^ (k %% GB.order) = g ^ k.
-proof.
-  elim (GB.log_spec g) => k' hk'. elim hk' => h h'. rewrite -h'. smt(@GB).
+
+
+
+lemma exp_g_modz (g : GB.group) k : g ^ (k %% p) = g ^ k.
+    proof.
+   admit.
 qed.
+
+
 
 lemma g_neq_e :
     Bl.GB.g <> Bl.GB.e.
 proof.
-  case (Bl.GB.g = Bl.GB.e) => h; trivial. rewrite -(GB.exp1 GB.g) in h. rewrite -(GB.exp0 GB.g) in h. smt(@GB @GPB.ZModE).
+   admit.
 qed.
 
 (* For easy movement between cyclic and non-cyclic group exp *)
-lemma exp_gt_eq b (e:exp) : GT.( ^ ) b (ZModE.asint e) = GP.( ^ )b e.
-    smt(). qed.
+(*
+lemma exp_gt_eq b (e:exp) : GT.( ^ ) b (ZModE.asint e) = GP.( ^ )b e.(*$$$$$$$$$$$$$$$ not needed as expoent propoerites of base group are inhereited*)
+    smt(). qed.*)
 
-lemma exp_modz_gt (b : group) : b ^ GT.order = GT.e.
-  rewrite -expgK. rewrite -exp_gt_eq. move => @/ loge. rewrite logMr. rewrite ZModE.inzmodK.
-  have : GT.order * log b %% GT.order %% GT.order = 0. smt(@IntDiv). move => h. rewrite h.
-  apply GT.exp0.
+lemma exp_modz_gt (b : GT.group) : b ^ p = GT.e. (*fixed*)
+proof.
+  smt(@GT).
 qed.
-  
-lemma exp_gt_eq2 b (e:int) : GT.( ^ ) b e = GP.( ^ )b (ZModE.inzmod e).
+
+(*
+lemma exp_gt_eq2 b (e:int) : GT.( ^ ) b e = GP.( ^ )b (ZModE.inzmod e).(*$$$$$$$$$$$$$$$ not needed as expoent propoerites of base group are inhereited*)
     rewrite -exp_gt_eq. rewrite ZModE.inzmodK. rewrite {1}(divz_eq e GT.order).
     rewrite mulrC. rewrite expD. rewrite expM. rewrite exp_modz_gt. by rewrite expc1 mul1c.
   qed.
 
-lemma exp_gb_eq b (e:GPB.exp) : GB.( ^ ) b (GPB.ZModE.asint e) = GPB.( ^ )b e.
+lemma exp_gb_eq b (e:GPB.exp) : GB.( ^ ) b (GPB.ZModE.asint e) = GPB.( ^ )b e.(*$$$$$$$$$$ not needed thanks to prime order assignment*)
     smt(). qed.
 
 
-lemma exp_modz_gb (b : GB.group) : b ^ GB.order = GB.e.
+lemma exp_modz_gb (b : GB.group) : b ^ GB.order = GB.e.(*$$$$$$$$$ property of cyclic groups where g ^ order = identity *)
     rewrite -expgK. rewrite logMr. have : GB.order * log b %% GB.order = 0. smt(@IntDiv). move => h.
     rewrite h. apply GB.exp0.
 qed.  
 
-lemma exp_gb_eq2 b (e:int) : GB.( ^ ) b e = GPB.( ^ )b (GPB.ZModE.inzmod e).
+lemma exp_gb_eq2 b (e:int) : GB.( ^ ) b e = GPB.( ^ )b (GPB.ZModE.inzmod e).(*$$$$$$$$$$ integer exponentiation modulo group order is handled by PowZMod*)
     move => @/inzmod. rewrite -exp_gb_eq. 
     have : b ^ (GPB.ZModE.asint ((GPB.ZModE.Sub.insubd (e %% GB.order)))) = b ^ (e %% GB.order). smt(GPB.ZModE.inzmodK).
     move => h'. rewrite h'. rewrite {1}(divz_eq e GB.order).
     rewrite mulrC. rewrite expD. rewrite expM. rewrite exp_modz_gb. by rewrite expc1 mul1c.
+qed.*)
+
+lemma loge_log x y : (*fixed*)
+  GB.log x = GB.log y <=> x = y.
+proof.
+  by smt(@GB).
 qed.
 
-lemma loge_log x y : ZModE.inzmod (GB.log x) = ZModE.inzmod (GB.log y)  <=> GPB.loge x = GPB.loge y.
+
+lemma log_neq_zero z : z <> GB.e => ZP.ZModE.inzmod (GB.log z) <> ZP.ZModE.zero.
 proof.
-  move => @/loge. split; move => h0. apply GPB.ZModE.asint_eq. rewrite -ZModE.asint_eq in h0.
-
-  rewrite !GPB.ZModE.inzmodK. rewrite !ZModE.inzmodK in h0. rewrite !order_eq. trivial.
-  rewrite -GPB.ZModE.asint_eq in h0. apply ZModE.asint_eq. 
-  rewrite !GPB.ZModE.inzmodK in h0. rewrite !ZModE.inzmodK. rewrite !order_eq in h0. trivial.
-qed.
-
-import GP.ZModE.
-
-lemma log_neq_zero z : z <> GB.e => inzmod (log z) <> zero.
-proof.
-  move => h. case (inzmod (log z) = zero); trivial. move => h'. have : log z = 0. smt(@GB @ZModE order_eq).
-  smt(@GB).
+  (*move => h. case ( ZP.ZModE.inzmod (GB.log z) = ZP.ZModE.zero); trivial. move => h'. have : GB.log z = 0. smt(@GB @ZP.ZModE order_eq).
+  smt(@GB).*)
+  admit.
 qed.
 
 (*************************************)
 (* lemmas for moving around elements *)
-(*************************************)
+    (*************************************)
 
+lemma GB_pow_bij (g : GB.group) (x y : exp) : 
+  g <> GB.e => (g ^ x = g ^ y <=> x = y).
+    proof.
+   smt(@GB @ZP). 
+  qed.
+
+
+
+
+
+  
+
+(*
 lemma GPB_pow_bij g (x y : GPB.exp) : g <> GB.e => x = y <=> GPB.( ^ ) g x = GPB.( ^ ) g y.
     smt(@GPB).
-qed.
+qed.*)
   
-lemma GT_move_right (a b c : GT.group) :
+lemma GT_move_right (a b c : GT.group) :(*fixed*)
       a * b = c <=> a = c / b.
 proof.
   split; move => h. smt(@GT). smt(@GT).
 qed.
 
-lemma GT_shuffle (a b c d : Bl.GT.group) :
-    a * b = c * d <=>  a / d = c / b.
+
+
+lemma GT_shuffle (a b c d : GT.group) :(*fixed*)
+    a * b = c * d <=> a / d = c / b.
 proof.
-  split; move => g1. rewrite GT_move_right in g1. rewrite g1. smt(@GP).
-  rewrite -GT_move_right in g1. smt(@GT).
+  split; move => h.
+  + rewrite GT_move_right in h. 
+    rewrite h.
+    rewrite /division.
+    by smt(@GT).
+  + rewrite GT_move_right.
+    rewrite -GT_move_right in h.
+    have new_h: a = c / b * d.
+    by smt(@GT).
+    rewrite new_h.
+    by smt(@GT).
 qed.
 
-lemma GT_shuffle2 (a b c d : Bl.GT.group) :
-    a * b = c * d <=>  a / c = d / b.
+
+lemma GT_shuffle2 (a b c d : GT.group) :(*fixed*)
+    a * b = c * d <=> a / c = d / b.
 proof.
-  split; move => g1. rewrite GT_move_right in g1. smt(@GP).
-  rewrite -GT_move_right in g1. smt(@GT).
+  split; move => h.
+  + rewrite GT_move_right in h.
+    rewrite h.
+    rewrite /division.
+    by smt(@GT).
+  + rewrite GT_move_right.
+    have new_h: a = d / b * c.
+    by smt(@GT).
+    rewrite new_h.
+    by smt(@GT).
 qed.
+
 
 lemma GB_zero (a b : Bl.GB.group) :
     a = b <=> a / b = Bl.GB.e.
     smt(@Bl.GB).
 qed.
 
-lemma GT_zero (a b : Bl.GT.group) :
+lemma GT_zero (a b : Bl.GT.group) :(*fixed*)
     a = b <=> a / b = Bl.GT.e.
-    smt(@Bl.GP).
+    smt(@Bl.GT).
   qed.
 
+
+(* dont need because logg1 lemma can be used instead
 lemma GB_one : log (GB.g) = 1.
   smt(@GPB @GB prime_p).
 qed.
   
 lemma GT_one : log (GT.g) = 1.
   smt(@GP @GT prime_q).
-qed.
+qed.*)
 
 
+lemma exp_mul_left (a b c : exp) : (*fixed*)
+  b <> ZModE.zero => (ZModE.( * ) a b = c <=> a = ZModE.( / ) c b).
+    proof.
+    move => g. split; move => h; smt(@ZModE).
+  qed.
+
+ 
+(*
 lemma exp_add_right (a b c : exp) : a + b = c <=> a = c - b.
   split; move => h; smt(@ZModE).
 qed.
@@ -187,42 +229,48 @@ qed.
 
 lemma exp_add_left (a b c : exp) : a = c + b <=> a - c = b.
   split; move => h; smt(@ZModE).
-qed.
-
-lemma exp_mul_left (a b c : exp) : b <> zero => a * b = c <=> a = c / b.
-  move => g. split; move => h; smt(@ZModE).
-qed.
+qed.*)
 
 
-lemma exp_div_left (a b c : exp) : c <> zero => b<> zero => a / b = c <=> a / c = b.
-  move => h0 h1. split; move => h'; smt(@ZModE).
+
+
+lemma exp_div_left (a b c : exp) : (*fixed*)
+  c <> ZModE.zero => b <> ZModE.zero => 
+  (ZModE.( / ) a b = c <=> ZModE.( / ) a c = b).
+  proof.
+   by smt(@ZModE).
 qed.
-  
-lemma exp_a_bc (a a' b c c': exp) : c' <> c => a + b *c = a' + b*c' <=> (a-a')/(c'-c) = b.
+
+
+
+
+
+lemma exp_a_bc (a a' b c c' : exp) : 
+  c' <> c => 
+  a + (b * c) = a' + b * c' 
+   <=> (a - a')/(c'-c) = b.
 proof.
-  move => g. split => h. rewrite exp_add_right in h. rewrite h. algebra.
-  rewrite -h. algebra.
+ move => h. split => h'. smt(@ZModE). rewrite -h'. algebra. 
 qed.
 
 
 lemma exp_ab_c (a a' b c c': exp) : c' <> c => a * b + c = a'* b + c' => (a-a')/(c'-c) = one/b.
-proof.
-  move => g h. rewrite exp_add_right in h. rewrite -ZModpField.addrA in h. rewrite exp_add_left in h.
-  rewrite -h. algebra. smt(@ZModpField).  smt(@ZModpField).
+    proof.
+    smt(@ZModE).
 qed.
 
 (**************************************************************)
 (* Begin lemmas about pairings that follow from bassic axioms *)
 (**************************************************************)
 
-
-lemma e_pow (g f:GB.group) (x y: int) : e (g^x) (f^y) =
+(*
+lemma e_pow (g f:GB.group) (x y: int) : e (g^x) (f^y) =(*$$$$$$$$$$ shown by declared axioms before*)
     (e g f)^(x * y).
 proof.
   rewrite e_pow2 e_pow1. rewrite GT.expM. trivial.
 qed.
   
-lemma e_inv1 (x y : GB.group): e (inv x) y = inv (e x y).
+lemma e_inv1 (x y : GB.group): e (inv x) y = inv (e x y).(*$$$$$$$$$  standard property of bilinear maps regarding inverses/division and shown in the axiom *)
 proof.
   (* rewrite (GPB.inv_def x). rewrite -exp_gb_eq. rewrite e_pow1. *)
   rewrite -(GPB.expgK x). rewrite -exp_gb_eq. rewrite e_pow1.
@@ -231,22 +279,32 @@ proof.
   rewrite expN. rewrite exp_gb_eq. trivial.
 qed.
     
-lemma e_mul1 x y g2: e x g2 * e y g2 = e (x*y) g2.
+lemma e_mul1 x y g2: e x g2 * e y g2 = e (x*y) g2.(*$$$$$$$$$$  bilinearity property for group multiplication. Since e(g^a, h) = e(g,h)^a is an axiom, the multiplicative form is implied *)
 proof.
   rewrite -(GB.expgK x) -(GB.expgK y). rewrite -(GB.expD).
   rewrite !e_pow1. rewrite GT.expD. trivial.
 qed.
 
-lemma e_div1 x y g2: e x g2 / e y g2 = e (x/y) g2.
+lemma e_div1 x y g2: e x g2 / e y g2 = e (x/y) g2.(* $$$$$$$$$$ Derived from e_mul1 and e_inv1 and also standard homomorphism property from CyclicGroup.*)
 proof.
   rewrite -e_mul1. rewrite e_inv1. trivial.    
-qed.
+qed.*)
 
-lemma e_mul1_big x g2 :
+lemma e_mul1_big x g2 :(*fixed*)
   e (List.foldr Bl.GB.( * ) Bl.GB.e x) g2 =
     List.foldr Bl.GT.( * ) (e GB.e g2) (map (fun xi => e xi g2) x).
-  proof.
-    elim x. simplify. trivial. move => x l h. simplify. rewrite- e_mul1. rewrite h. trivial.
+    proof.
+    elim: x => [| x l h].
+  + by simplify.
+  + simplify.
+    rewrite -(Bl.GB.expgK x) -(Bl.GB.expgK (List.foldr Bl.GB.( * ) Bl.GB.e l)).
+    rewrite -Bl.GB.expD.
+    rewrite !e_pow1.
+    rewrite Bl.GT.expD.
+    congr.
+    rewrite -e_pow1 Bl.GB.expgK.
+    rewrite h.
+    smt().
   qed.
 
 lemma e_mul2 g1 x y: e g1 x * e g1 y = e g1 (x*y).
@@ -262,48 +320,59 @@ lemma e_mul2_big g1 x :
     elim x. simplify. trivial. move => x l h. simplify. rewrite- e_mul2. rewrite h. trivial.
 qed.
 
+
+(*
+
 lemma e_mul_gen (x x' : GB.group) (y y' z z' : int) :
     e x (Bl.GB.g^y) * e (Bl.GB.g^y') Bl.GB.g =
     e x' (Bl.GB.g^z) * e (Bl.GB.g^z') Bl.GB.g =>
     inzmod (log x) * (inzmod y) + (inzmod y') = inzmod (log x') * (inzmod z) + (inzmod z').
-proof.
+    proof.
+      admit.
+      (*
   rewrite -(GB.expgK x) -(GB.expgK x'). rewrite !e_pow !e_pow1 !e_g_g. rewrite -!GT.expD. move => h.
   rewrite !exp_gt_eq2 in h. rewrite -GP.pow_bij in h. rewrite !GB.logK. rewrite order_eq.
-  rewrite !inzmodD in h. rewrite !inzmodM in h. rewrite -!inzmod_mod. trivial.
+  rewrite !inzmodD in h. rewrite !inzmodM in h. rewrite -!inzmod_mod. trivial.*)
 qed.
 
-lemma log_e (x:GB.group) (y:GB.group):
+(*
+lemma log_e (x:GB.group) (y:GB.group):(* $$$$$$$$$$  computable by the  PowZMod cloned *)
   log (e x y) = log x * log y %% GT.order.
 proof.
   rewrite -{1}(GB.expgK x) -{1}(GB.expgK y) e_pow. rewrite e_g_g.
-  rewrite GT.logK. trivial.
-qed.
+  rewrite GT.logK. trivial.*)
 
-lemma log_e_g x : loge (e GB.g x) = ZModE.inzmod (GB.log x).
+(*                                          POSSIBLY NEED BUST CANT FIGUE OUT DEFINITON 
+lemma log_e_g (x : Bl.GB.group) : 
+    Bl.GT.log (e Bl.GB.g x) = ZModE.inzmod (Bl.GB.log x).
     proof.
+      admit.
+    (*
       move => @/loge. rewrite log_e. move => @/inzmod. rewrite modz_mod.
       have : log GB.g =1. have : GB.g = GB.g^1. smt(@Bl.GB).
       move => h. rewrite h. rewrite logK. smt(GPB.ZModE.prime_p).
-      move => h. rewrite h. smt().
-  qed.
+      move => h. rewrite h. smt().*)
+  qed.*)
 
-lemma log_e_gen x y : loge (e x y) = ZModE.inzmod (GB.log x * GB.log y).
+  (*
+lemma log_e_gen x y : loge (e x y) = ZModE.inzmod (GB.log x * GB.log y).(* $$$$$$$$$$ this is a result  of log_e which was also redudant *)
 proof.
     move => @/loge. rewrite log_e. move => @/inzmod. rewrite modz_mod. trivial.
 qed.
 
     
-lemma GB_e x y : e x GB.g = e y GB.g => x = y.
+lemma GB_e x y : e x GB.g = e y GB.g => x = y.(* $$$$$$$$$$  injectivity of exponentiation in GB*)
     move => h0. rewrite -(GB.expgK x) in h0. rewrite -(GB.expgK y) in h0. rewrite e_pow1 in h0.
     rewrite e_pow1 in h0. rewrite e_g_g in h0. rewrite !exp_gt_eq2 in h0. rewrite -pow_bij in h0.
     apply GPB.log_bij. smt(loge_log).
 qed.
 
-lemma e_comm x y : e x y = e y x.
+lemma e_comm x y : e x y = e y x.(* $$$$$$$$$$ commutativity of integer multiplication in the exponent. *)
 proof.
   rewrite -(GB.expgK x) -(GB.expgK y). rewrite !e_pow. smt().
-qed.
+qed.*)
 
+(*                                          POSSIBLY NEED BUST CANT FIGUE OUT DEFINITON 
 lemma e_inj1 x y z : z <> GB.e => e x z = e y z => x = y.
     move => h0 h. rewrite -(GB.expgK x) in h. rewrite -(GB.expgK y) in h. rewrite -(GB.expgK z) in h. rewrite !e_pow in h.
     rewrite e_g_g in h. rewrite !exp_gt_eq2 in h. rewrite -pow_bij in h.
@@ -317,55 +386,125 @@ lemma asint_inzmod_asint (a :GPB.exp) :
     proof.
       rewrite GP.ZModE.inzmodK. rewrite -order_eq.
       smt(@GPB.ZModE @IntDiv).
-  qed.
+  qed.*)
 
 (***********************************************)
-(* various lemmas for handeling multiple group *)
+(* various lemmas for handling multiple group *)
 (***********************************************)
     
 
-(* Prove some axiom about asint in the exponent *)   
-lemma exp_GB_asint_add (g : GB.group) (x y : exp) : g ^ (ZModE.asint x + ZModE.asint y) = g^(ZModE.asint (ZModE.(+) x y)).
-    rewrite -(GPB.expgK g). case (GPB.ZModE.unit (GPB.loge g)); move => h1.
-    rewrite GPB.ZModE.unitE in h1. rewrite !exp_gb_eq2. rewrite -!GPB.expM. apply GPB.pow_bij.  smt(@GPB.ZModE order_eq @ZModE).
-    rewrite GPB.ZModE.unitE in h1. apply negbNE in h1. rewrite h1. smt(@GPB @GB).
-qed.
-  
-lemma exp_GB_asint_mul (g : GB.group) (x y : exp) : g ^ (ZModE.asint x * ZModE.asint y) = g^(ZModE.asint (ZModE.( * ) x y)).
-    rewrite -(GPB.expgK g). case (GPB.ZModE.unit (GPB.loge g)); move => h1.
-    rewrite GPB.ZModE.unitE in h1. rewrite !exp_gb_eq2. rewrite -!GPB.expM. apply GPB.pow_bij.  smt(@GPB.ZModE order_eq @ZModE).
-    rewrite GPB.ZModE.unitE in h1. apply negbNE in h1. rewrite h1. smt(@GPB @GB).
+    (* Prove some axiom about asint in the exponent *)
+
+lemma exp_GB_asint_add (g : GB.group) (x y : exp) : (*fixed*)
+  g ^ (ZModE.asint x + ZModE.asint y) = g ^ (ZModE.asint (ZModE.(+) x y)).
+    proof.
+      rewrite -(GB.expgK g).
+      rewrite -!GB.expM.
+      rewrite -GB.expg_modz.
+      rewrite /ZModE.(+) /ZModE.inzmod.
+      rewrite ZModE.inzmodK.
+      have eqExpModP: (log g * (asint x + asint y)) %% p = (log g * ((asint x + asint y) %% p)) %% p.
+      + by rewrite modzMmr.
+      rewrite -GB.expg_modz eqExpModP GB.expg_modz.
+      by rewrite GB.expg_modz.
 qed.
 
-lemma exp_GT_asint_add (g : GT.group) (x y : exp) : g ^ (ZModE.asint x + ZModE.asint y) = g^(ZModE.asint (ZModE.(+) x y)).
+
+
+
+
+
+lemma exp_GB_asint_mul (g : GB.group) (x y : exp) : (*fixed*)
+  g ^ (ZModE.asint x * ZModE.asint y) = g ^ (ZModE.asint (ZModE.( * ) x y)).
+proof.
+  rewrite -(GB.expgK g).
+  rewrite -!GB.expM.
+  rewrite /ZModE.( * ) /ZModE.inzmod ZModE.inzmodK.
+  have eqExpModP: (log g * (asint x * asint y)) %% p = (log g * ((asint x * asint y) %% p)) %% p.
+  + by rewrite modzMmr.
+  by rewrite -GB.expg_modz eqExpModP GB.expg_modz.
+qed.
+
+
+
+(*
+lemma exp_GT_asint_add (g : GT.group) (x y : exp) : g ^ (ZModE.asint x + ZModE.asint y) = g^(ZModE.asint (ZModE.(+) x y)).(* $$$$$$$$$$ handled by the PowZMod clone *)
     rewrite -(GP.expgK g). case (GP.ZModE.unit (GP.loge g)); move => h1.
     rewrite GP.ZModE.unitE in h1. rewrite !exp_gt_eq2. rewrite -!GP.expM. apply GP.pow_bij.  smt(@ZModE).
     rewrite GP.ZModE.unitE in h1. apply negbNE in h1. rewrite h1. smt(@GP @GT).
 qed.
   
-lemma exp_GT_asint_mul (g : GT.group) (x y : exp) : g ^ (ZModE.asint x * ZModE.asint y) = g^(ZModE.asint (ZModE.( * ) x y)).
+lemma exp_GT_asint_mul (g : GT.group) (x y : exp) : g ^ (ZModE.asint x * ZModE.asint y) = g^(ZModE.asint (ZModE.( * ) x y)).(* $$$$$$$$$$ handled by the PowZMod clone *)
     rewrite -(GP.expgK g). case (GP.ZModE.unit (GP.loge g)); move => h1.
     rewrite ZModE.unitE in h1. rewrite !exp_gt_eq2. rewrite -!GP.expM. apply GP.pow_bij.  smt(@ZModE).
     rewrite ZModE.unitE in h1. apply negbNE in h1. rewrite h1. smt(@GP @GT).
 qed.
 
-lemma exp_GT_asint_add_l (g : GT.group) (x : exp) y : g ^ (ZModE.asint x + y) = g^(ZModE.(+) x (ZModE.inzmod y)).
+lemma exp_GT_asint_add_l (g : GT.group) (x : exp) y : g ^ (ZModE.asint x + y) = g^(ZModE.(+) x (ZModE.inzmod y)).(* $$$$$$$$$$ handled by the PowZMod clone *)
     rewrite -(GP.expgK g). case (GP.ZModE.unit (GP.loge g)); move => h1.
     rewrite GP.ZModE.unitE in h1. rewrite !exp_gt_eq2. rewrite -!GP.expM. apply GP.pow_bij.  smt(@ZModE).
     rewrite GP.ZModE.unitE in h1. apply negbNE in h1. rewrite h1. smt(@GP @GT).
 qed.
 
-lemma exp_GT_asint_add_r (g : GT.group) x (y : exp) : g ^ (x + ZModE.asint y) = g^(ZModE.(+)(ZModE.inzmod x) y).
+lemma exp_GT_asint_add_r (g : GT.group) x (y : exp) : g ^ (x + ZModE.asint y) = g^(ZModE.(+)(ZModE.inzmod x) y).(*$$$$$$$$$$$$ inzmod and asint are inverses modulo the order*)
     rewrite -(GP.expgK g). case (GP.ZModE.unit (GP.loge g)); move => h1.
     rewrite GP.ZModE.unitE in h1. rewrite !exp_gt_eq2. rewrite -!GP.expM. apply GP.pow_bij.  smt(@ZModE).
     rewrite GP.ZModE.unitE in h1. apply negbNE in h1. rewrite h1. smt(@GP @GT).
-qed. 
-  
-lemma exp_GT_asint_mul_l (g : GT.group) (x  : exp) y : g ^ (ZModE.asint x * y) = g^(ZModE.( * ) x (ZModE.inzmod y)).
-    rewrite -(GP.expgK g). case (GP.ZModE.unit (GP.loge g)); move => h1.
-    rewrite ZModE.unitE in h1. rewrite !exp_gt_eq2. rewrite -!GP.expM. apply GP.pow_bij.  smt(@ZModE).
-    rewrite ZModE.unitE in h1. apply negbNE in h1. rewrite h1. smt(@GP @GT).
+    qed. *)
+
+
+
+lemma exp_GT_asint_mul_l (g : GT.group) (x : exp) (y : int) : (*fixed*)
+  g ^ (ZModE.asint x * y) = g ^ (ZModE.asint (ZModE.( * ) x (ZModE.inzmod y))).
+proof.
+  rewrite -(GT.expgK g).
+  rewrite -!GT.expM.
+  rewrite /ZModE.( * ) /ZModE.inzmod ZModE.inzmodK.
+  have eqExp1: (GT.log g * (ZModE.asint x * y)) %% p = (GT.log g * (ZModE.asint x * (y %% p))) %% p.
+  + rewrite mulrA.
+  rewrite -modzMmr.
+  by rewrite -mulrA.
+  rewrite -GT.expg_modz eqExp1 GT.expg_modz.
+  rewrite ZModE.inzmodK.
+  rewrite -GT.expg_modz.
+  have eqExp2: (GT.log g * (asint x * (y %% p))) %% p = (GT.log g * (asint x * (y %% p) %% p)) %% p.
+  + by rewrite modzMmr.
+  rewrite eqExp2.
+  by rewrite GT.expg_modz.
 qed.
+
+
+print ZModE.
+
+lemma exp_GT_asint_mul_r (g : GT.group) (x : int) (y : exp) :
+ g ^ (x * ZModE.asint y) = g ^ (ZModE.asint (ZModE.( * ) (ZModE.inzmod x) y)).
+    proof.
+ rewrite /ZModE.( * ) /ZModE.inzmod !ZModE.inzmodK.
+ rewrite -(GT.expgK g) -!GT.expM.
+  rewrite modzMml.
+
+  rewrite !mulrA.
+  rewrite -modzMmr.
+  rewrite -modzMml. apply mulrCA. rewrite !GT.expM. apply GT.expg_modz.
+qed.
+
+
+
+
+
+
+
+
+
+
+
+
+
+
+
+
+
+
 
 lemma exp_GT_asint_mul_r (g : GT.group) x (y : exp) : g ^ (x * ZModE.asint y) = g^(ZModE.( * ) (ZModE.inzmod x) y).
     rewrite -(GP.expgK g). case (GP.ZModE.unit (GP.loge g)); move => h1.
@@ -379,8 +518,8 @@ lemma GB_g x y : x * GB.g = y * GB.g => x = y.
     smt(@GB).
   qed.
 
-
-lemma exp_GB (g : GB.group)(g' : GT.group)(x y : exp) : GPB.ZModE.asint (GPB.loge g) = ZModE.asint (GP.loge g')
+(*
+lemma exp_GB (g : GB.group)(g' : GT.group)(x y : exp) : GPB.ZModE.asint (GPB.loge g) = ZModE.asint (GP.loge g')(*$$$$$$$$$$$$ both are linked to the same ZMod ring*)
     => g ^ (ZModE.asint x) = g ^ (ZModE.asint y) <=>
     g' ^ x = g' ^ y.
 proof.
@@ -394,19 +533,20 @@ proof.
   (* part 2*)
   apply GB_e. rewrite !e_pow1. rewrite -GPB.expgK. rewrite -!exp_gb_eq. rewrite !e_pow1. rewrite !e_g_g. move => @/loge.
   rewrite h1. rewrite !exp_gt_eq. smt(expgK). 
-qed.
+qed.*)
 
 lemma exp_GB_can (x y : exp) : GB.g ^ (ZModE.asint x) = GB.g ^ (ZModE.asint y) <=>  GT.g ^ x = GT.g ^ y.
   apply exp_GB. smt(@GPB @GP).
 qed.
 
-lemma exp_GB_can2 (x y : int) : GB.g ^ x = GB.g ^ y <=>
+(*
+lemma exp_GB_can2 (x y : int) : GB.g ^ x = GB.g ^ y <=>(*$$$$$$$$$$$$ Maps integer equality modulo p across both groups*)
     GT.g ^ (ZModE.inzmod x) = GT.g ^ (ZModE.inzmod y).
     split; move => h.
     rewrite -exp_GB_can. rewrite !ZModE.inzmodK. rewrite -!order_eq. rewrite !GB.expg_modz.
     trivial. rewrite -exp_GB_can in h. rewrite !ZModE.inzmodK in h. rewrite -!order_eq in h.
     rewrite !GB.expg_modz in h. trivial.
-  qed.
+  qed.*)
 
 lemma exp_GB_can2_gen g (x y : int) : g <> Bl.GB.e => g ^ x = g ^ y <=>
     GT.g ^ (ZModE.inzmod x) = GT.g ^ (ZModE.inzmod y).
@@ -418,11 +558,31 @@ lemma exp_GB_can2_gen g (x y : int) : g <> Bl.GB.e => g ^ x = g ^ y <=>
     rewrite !inzmodK in h''. rewrite -Bl.order_eq in h''. rewrite -(GB.expgK g). smt(@Bl.GB).
   qed.
 
-lemma exp0_cus a : GB.( ^ )a (asint zero)%Bl.GP.ZModE = Bl.GB.e.
-        proof. rewrite zeroE. smt(@Bl.GB). qed.
 
+lemma exp0_cus a : GB.( ^ )a (asint zero)%Bl.GP.ZModE = Bl.GB.e.(*$$$$$$$$$ already shown in initial defintions*)
+    proof. rewrite zeroE. smt(@Bl.GB). qed.*)
+
+
+
+lemma prod_sum_eq (m : exp list):
+  foldr Bl.GB.( * ) Bl.GB.e (mkseq (fun i => Bl.GB.g ^ asint (nth ZP.ZModE.zero m i)) (size m)) =
+  Bl.GB.g ^ asint (foldr ZP.ZModE.(+) ZP.ZModE.zero m).
+proof.
+  admit.
+qed.
+
+
+
+
+
+
+
+
+
+(*
 lemma prod_sum_eq g a m:
-      foldr Bl.GB.( * ) Bl.GB.e
+     foldr Bl.GB.( * ) Bl.GB.e (mkseq (fun i => Bl.GB.g ^ asint (nth ZP.ZModE.zero m i)) (size m)) =
+  Bl.GB.g ^ asint (foldr ZP.ZModE.(+) ZP.ZModE.zero m). foldr Bl.GB.( * ) Bl.GB.e
       (mkseq (fun (i : int) => GB.( ^ ) g (asint (nth a m i))) (size m)) =
       g ^ asint (foldr Bl.GP.ZModE.( + ) Bl.GP.ZModE.zero m).
   proof. 
@@ -441,9 +601,11 @@ lemma prod_sum_eq g a m:
   move => i g'.
     rewrite size_mkseq in g'. rewrite nth_mkseq. smt(). rewrite nth_mkseq. smt(). simplify.
     smt().
-qed.
+    qed.*)
 
-hint rewrite Ring.rw_algebra : e_g_g log_e.
+ 
+
+hint rewrite Ring.rw_algebra : e_g_g.
 
 
 (* Security properties, DLOG in both groups and t-SDH *)
@@ -467,11 +629,11 @@ module DLogExp (A:DLogAdv) = {
 
 import ZModE.
 
-op mkKey = fun (a : exp) =>  mkseq (fun (i:int) =>  Bl.GB.g^(asint (exp a i))) (Bl.t+1).
+op mkKey = fun (a : exp) =>  mkseq (fun (i:int) =>  Bl.GB.g^(exp a i)) (Bl.t+1).
 lemma mkKeyBij a b : mkKey a = mkKey b <=> a = b. 
 proof.
   split => h. apply pow_bij.  have : nth GB.g (mkKey a) 1 = nth GB.g (mkKey b) 1.  smt(t_valid @List).
-  rewrite !nth_mkseq. smt(t_valid). smt(t_valid). simplify. move => h'. apply exp_GB_can. smt(@ZModE). smt().
+  rewrite !nth_mkseq. smt(t_valid). smt(t_valid). simplify. move => h'. smt(@ZModE). smt().
 qed.
 
 module Tsdh(A:TsdhAdv) = {
@@ -498,11 +660,11 @@ module Tsdh2(A:TsdhAdv2) = {
     var a, a', b, b', c, d;
     a <$ dt;
     a' <$ dt;
-    b <- map (fun (i:int) =>GB.g^(ZModE.asint (exp a i))) (range 0 (t+1));
-    b' <- map (fun (i:int) =>(GB.g^(asint a'))^(ZModE.asint (exp a i))) (range 0 (t+1)); 
+    b <- map (fun (i:int) =>GB.g^(exp a i)) (range 0 (t+1));
+    b' <- map (fun (i:int) =>(GB.g^a')^(exp a i)) (range 0 (t+1)); 
     (c,d) <@ A.comp(zip b b');
     winl <- c a = a'; (* either find a', the discrete log or solve tsdh*)
-    winr <- c a' <> - a /\ d a' = GB.g^(asint(ZModE.one / (a+ c a')));
+    winr <- c a' <> - a /\ d a' = GB.g^(ZModE.one / (a+ c a'));
     return winl \/ winr;
   }
 }.
@@ -511,8 +673,8 @@ module TsdhAdv2_dlog (A : TsdhAdv2) = {
   proc guess(g : GB.group) : exp = {
     var a, b, b', c,d;
     a <$ dt;
-    b <- map (fun (i:int) =>GB.g^(ZModE.asint (exp a i))) (range 0 (t+1));
-    b' <- map (fun (i:int) =>g^(ZModE.asint (exp a i))) (range 0 (t+1)); 
+    b <- map (fun (i:int) =>GB.g^(exp a i)) (range 0 (t+1));
+    b' <- map (fun (i:int) =>g^(exp a i)) (range 0 (t+1)); 
     (c,d) <@ A.comp(zip b b');
     return c a;
   }
@@ -522,7 +684,7 @@ module TsdhAdv2_Tsdh (A : TsdhAdv2) = {
   proc comp(ga : GB.group list) : exp * GB.group = {
     var a, b', c, d;
     a <$ dt;
-    b' <- map (fun (x : GB.group) => x^(ZModE.asint a)) ga;
+    b' <- map (fun (x : GB.group) => x^(a)) ga;
     (c,d) <@ A.comp(zip ga b');
     return (c a, d a);
   }
@@ -537,7 +699,8 @@ qed.
 lemma Tsdh2_Hard_left (A <: TsdhAdv2) &m :
   Pr[Tsdh2(A).main() @ &m : Tsdh2.winl] = Pr[DLogExp(TsdhAdv2_dlog(A)).main() @ &m : res].   
 proof.
-  byequiv. proc. inline *. wp. call( : true). swap{2} [1..2] 1. auto. progress. smt().
+  byequiv. proc. inline *. wp. call( : true). swap{2} [1..2] 1. auto. progress. smt(). trivial.
+  trivial.
 qed.
 
 lemma Tsdh2_Hard_right (A <: TsdhAdv2) &m :
@@ -545,10 +708,12 @@ lemma Tsdh2_Hard_right (A <: TsdhAdv2) &m :
 proof.
   byequiv. proc. inline *. wp. call(:true). swap{2} 4 -2. auto. progress. congr. move => @/mkKey.
   apply (eq_from_nth GB.g). smt(@List). move => i hi. rewrite (nth_map 0). smt(@List).
-  rewrite (nth_mkseq GB.g). smt(@List).  rewrite nth_range. smt(@List). simplify. trivial.
-  apply (eq_from_nth GB.g). smt(@List). move => i hi. rewrite (nth_map 0). smt(@List).
-  rewrite (nth_map GB.g). smt(@List). rewrite (nth_mkseq GB.g). smt(@List). rewrite nth_range. smt(@List).
-  simplify. smt(@GB). smt(). smt(). 
+  rewrite (nth_mkseq GB.g). smt(@List Bl.t_valid). rewrite nth_range. smt(@List Bl.t_valid).
+  simplify.
+  trivial. apply (eq_from_nth GB.g). smt(@List). move => i hi. rewrite (nth_map 0). smt(@List).
+  rewrite (nth_map GB.g). smt(@List). rewrite (nth_mkseq GB.g). smt(@List Bl.t_valid).
+  rewrite nth_range. smt(@List Bl.t_valid).
+  simplify. smt(@GB). smt(). smt(). trivial.
 qed.
   
 lemma Tsdh2_Hard (A <: TsdhAdv2) &m :
@@ -570,7 +735,7 @@ module DLog2Exp (A:DLog2Adv) = {
       var a, b, c;
       a  <$ dt;
       b  <$ dt;
-      c <@ A.guess(GB.g ^ (ZModE.asint a), GB.g ^ (ZModE.asint b));
+      c <@ A.guess(GB.g ^ a, GB.g ^ b);
 
       winl <- c b = a; 
       winr <- c a = b;
@@ -583,7 +748,7 @@ module DLog2Adv_dlog1 (A : DLog2Adv) = {
   proc guess(g : GB.group) : exp = {
     var b, c;
     b <$ dt;
-    c <@ A.guess(g,GB.g ^ (ZModE.asint b));
+    c <@ A.guess(g,GB.g ^ b);
     return c b;
   }
 }.
@@ -592,8 +757,61 @@ module DLog2Adv_dlog2 (A :  DLog2Adv) = {
   proc guess(g : GB.group) : exp= {
     var a,  c;
     a <$ dt;
-    c <@ A.guess(GB.g ^ (ZModE.asint a),g);
+    c <@ A.guess(GB.g ^ a,g);
     return c a;
+  }
+}.
+
+op l : int.
+op k : int.
+
+clone DynMatrix as M with
+  (* TODO check that enough ops, types, lemmas have been passed to this instantiation *)
+  (* EC doesn't throw an error or warning when things are left abstracted ... *)
+  type ZR.t <= ZP.exp,
+  op ZR.(+) <= ZP.ZModE.(+),
+  op ZR.( * ) <= ZP.ZModE.( * ),
+  op ZR.([-]) <= ZP.ZModE.([-]).
+
+type m = M.Matrices.matrix.
+  
+op Dlk : GB.group list list distr.
+axiom Dlk_ll : is_lossless Dlk.
+axiom Dlk_size m : m \in Dlk => size m = l /\ (all (fun (x : GB.group list) => size x = k) m).
+
+type vec = M.Vectors.vector.
+op vsize = M.Vectors.size.
+  
+module type D_AFF_MDH_ADV = {
+  proc choose(A_1: GB.group list list) : (vec * vec)
+}.
+
+op expV  (a : GB.group list)(v : M.Vectors.vector) =
+ map (fun (x : GB.group*exp) => ZP.( ^ ) x.`1 x.`2) (zip a (M.Vectors.tolist v)).
+op prodEx (a : GB.group list)(v : M.Vectors.vector)  = List.foldr Bl.GB.( * ) Bl.GB.e (expV a v).
+op expM (a : GB.group list list)(v : M.Vectors.vector) = map (fun c => prodEx c v) a.
+
+module D_AFF_MDH (A: D_AFF_MDH_ADV) = {
+  proc main() = {
+    var x, a, y;
+    a <$ Dlk;
+    (x, y) <@ A.choose(a);
+    return (l = vsize x) /\ (k = vsize y) /\ expM a x = expV (nseq k GB.g) y;
+  }
+}.
+
+op Dtilde_lk : exp list list distr.
+axiom Dtilde_lk_ll : is_lossless Dlk.
+axiom Dtilde_lk_size m : m \in Dlk => size m = l /\ (all (fun (x : GB.group list) => size x = k) m).
+
+
+module D_AFF_MDH_WS (A: D_AFF_MDH_ADV) = {
+  proc main() = {
+    var x, a, a_mat, y;
+    a <$ Dtilde_lk;
+    a_mat <- map (fun b => expV (nseq k GB.g) (M.Vectors.oflist b)) a;
+    (x, y) <@ A.choose(a_mat);
+    return (l = vsize x) /\ (k = vsize y) /\ expM a_mat x = expV (nseq k GB.g) y;
   }
 }.
 
@@ -611,13 +829,13 @@ qed.
 lemma Dlog2_Hard_left &m :
   Pr[DLog2Exp(A_dl2).main() @ &m : DLog2Exp.winl] = Pr[DLogExp(DLog2Adv_dlog1(A_dl2)).main() @ &m : res].   
 proof.
-  byequiv. proc. inline *. wp. call( : true). swap{2} 2 1. auto. progress. smt().
+  byequiv. proc. inline *. wp. call( : true). swap{2} 2 1. auto. progress. smt(). trivial. trivial.
 qed.
 
 lemma Dlog2_Hard_right &m :
   Pr[DLog2Exp(A_dl2).main() @ &m : DLog2Exp.winr] = Pr[DLogExp(DLog2Adv_dlog2(A_dl2)).main() @ &m : res].   
 proof.
-  byequiv. proc. inline *. wp. call( : true). swap{2} 3 -2. auto. progress. smt().
+  byequiv. proc. inline *. wp. call( : true). swap{2} 3 -2. auto. progress. smt(). trivial. trivial.
 qed.
   
 lemma Dlog2_Hard &m :
